ELMO: squashed

VLSM/Validating.v
@@ -25,7 +25,7 @@ Context
 
 (**
 We say that the component <<i>> of X is validating received messages if
-non-[projection_valid]itiy implied non-component-[valid]ity (or non-reachability).
+non-[projection_valid]itiy implied non-component-[valid]ity.
 *)
 
 Definition validating_projection_received_messages_prop
@@ -37,8 +37,7 @@ Definition validating_projection_received_messages_prop
 (**
 We can slightly generalize the definition above to also include empty messages
 and state it in a positive manner as the [validating_projection_prop]erty below,
-requiring that [valid]ity in the component (for reachable states) implies
-[projection_valid]ity.
+requiring that [valid]ity in the component implies [projection_valid]ity.
 *)
 
 Definition validating_projection_prop :=
@@ -46,67 +45,121 @@ Definition validating_projection_prop :=
         protocol_valid (pre_loaded_with_all_messages_vlsm (IM i)) li siomi ->
         vvalid Xi li siomi.
 
-(** An alternative formulation of the above property with a seemingly
-stronger hypoyesis, states that component (IM i) is validating for constraint
-if for any @si@ protocol state in the projection @Xi@, @li valid (IM i) (si, om)@
-implies  that there exists a state @s@ whose ith  component is @si@,
-and @s@ and @om@ are protocol in @X@, and @(i,li) valid (s,om)@ in @X@, that is,
-we have that @li valid (si, om)@ in the projection @Xi@.
-*)
-Definition validating_projection_prop_alt :=
-    forall (li : vlabel (IM i)) (siom : vstate (IM i) * option message),
-        let (si, om) := siom in
-        vvalid (IM i) li siom ->
-        protocol_state_prop Xi si ->
-        vvalid Xi li siom.
+Definition lifted_state_satisfying_constraint
+  (li : vlabel (IM i)) (si : vstate (IM i)) (om : option message) (s : vstate X) : Prop
+  := protocol_state_prop X s /\ s i = si /\  constraint (existT _ i li) (s, om).
 
-(** Under validating assumptions, all reachable states for component @IM i@ are
-protocol states in the projection @Xi@.
-*)
-Lemma validating_alt_free_states_are_projection_states
-    : validating_projection_prop_alt ->
-    forall s,
-        protocol_state_prop (pre_loaded_with_all_messages_vlsm (IM i)) s ->
-        protocol_state_prop Xi s.
+Definition valid_subsumes_constraint_prop : Prop :=
+  forall (li : vlabel (IM i)) (si : vstate (IM i)) (om : option message),
+    protocol_valid (pre_loaded_with_all_messages_vlsm (IM i)) li (si, om) ->
+    exists (s : vstate X), lifted_state_satisfying_constraint li si om s.
+
+Lemma validating_projection_prop_impl_valid_subsumes_constraint_prop :
+  validating_projection_prop -> valid_subsumes_constraint_prop.
 Proof.
-    intros Hvalidating s Hs.
-    induction Hs using protocol_state_prop_ind;
-    [apply initial_is_protocol;assumption|].
-    change s' with (fst (s',om')).
-    destruct Ht as [[_ [_ Hvalid]] Htrans].
-    rewrite <- Htrans.
-    apply (projection_valid_implies_destination_projection_protocol_state IM constraint i).
-    apply (Hvalidating l (s,om));assumption.
+  intros Hvalidating.
+  intros li si om Hv.
+  apply Hvalidating in Hv.
+  destruct Hv as [s [Heq [Hs [_ [_ Hc]]]]].
+  exists s. repeat split; assumption.
 Qed.
 
-(** Below we show that the two definitions above are actually equivalent.
-*)
-Lemma validating_projection_prop_alt_iff
-    : validating_projection_prop_alt <-> validating_projection_prop.
+Definition valid_message_is_protocol_in_composition_prop : Prop :=
+  forall
+  (om : option message)
+  (li : vlabel (IM i))
+  (si : vstate (IM i)),
+  protocol_valid (pre_loaded_with_all_messages_vlsm (IM i)) li (si, om) ->
+  option_protocol_message_prop X om.
+
+
+Lemma validating_projection_prop_impl_valid_message_is_protocol_in_composition_prop:
+  validating_projection_prop -> valid_message_is_protocol_in_composition_prop.
 Proof.
-    split.
-    - intros Hvalidating l (si, om) Hvalid.
-      destruct Hvalid as [Hsi [_ Hvalid]].
-      apply validating_alt_free_states_are_projection_states in Hsi
-      ; [|assumption].
-      exact (Hvalidating l (si,om) Hvalid Hsi).
-    - intros Hvalidating l (si, om) Hvalid HXisi.
-      specialize (Hvalidating l (si, om)).
-      apply Hvalidating.
-      repeat split; [| apply any_message_is_protocol_in_preloaded | assumption].
-      revert HXisi.
-      apply VLSM_incl_protocol_state.
-      apply proj_pre_loaded_with_all_messages_incl.
+  intros Hvalidating mi li si Hpv.
+  unfold validating_projection_prop in Hvalidating.
+  specialize (Hvalidating li (si, mi) Hpv).
+  clear Hpv.
+  unfold vvalid in Hvalidating. simpl in Hvalidating.
+  destruct Hvalidating as [s [Hsi [Hpsp [Hopmp Hccv]]]].
+  inversion Hopmp.
+  unfold protocol_message_prop.
+  exists x. apply H.
 Qed.
 
-Lemma validating_free_states_are_projection_states
-    : validating_projection_prop ->
-    forall s,
-        protocol_state_prop (pre_loaded_with_all_messages_vlsm (IM i)) s ->
-        protocol_state_prop Xi s.
+
+Lemma lift_reachability_to_protocol :
+  valid_subsumes_constraint_prop ->
+  valid_message_is_protocol_in_composition_prop ->
+  forall si,
+  protocol_state_prop (pre_loaded_with_all_messages_vlsm (IM i)) si ->
+  exists s, s i = si /\ protocol_state_prop (composite_vlsm IM constraint) s.
 Proof.
-    rewrite <- validating_projection_prop_alt_iff.
-    apply validating_alt_free_states_are_projection_states.
+      intros Hcp Hpcp si Hsi.
+      apply protocol_state_prop_iff in  Hsi.
+      destruct Hsi as [[[s Hs] Heq] | [l [(s, om) [om' Ht]]]]. 
+      - simpl in Heq. subst si. exists (lift_to_composite_state IM i s).
+        unfold lift_to_composite_state. rewrite state_update_eq.
+        split; [reflexivity|].
+        apply initial_is_protocol.
+        intro n.
+        destruct (decide (n = i)).
+        + subst n. rewrite state_update_eq. assumption.
+        + rewrite state_update_neq by assumption.  apply (proj2_sig (vs0 (IM n))).
+      - destruct Ht as [Hv Ht].
+        apply Hcp in Hv as Hcpv.
+        apply Hpcp in Hv as Hpcpv.
+        destruct Hcpv as [s0 [Hs0 [Heq Hc]]].
+        destruct (composite_transition IM (existT _ i l) (s0, om)) as (s', _om') eqn:Hct.
+        exists s'.
+        split.
+        + simpl in Hct. rewrite Heq in Hct.
+          match type of Hct with
+          | (let (_,_) := ?t in _) = _ => replace t with (si, om') in Hct
+          end.
+          inversion Hct.
+          subst _om' s'. clear Hct.
+          rewrite state_update_eq.
+          reflexivity.
+        + apply protocol_state_prop_iff. right.
+          exists (existT _ i l), (s0, om), _om'.
+          split; [|assumption].
+          destruct Hv as [_ [_ Hv]].
+          repeat split; try assumption.
+          simpl. rewrite Heq. assumption.
+Qed.
+
+
+Lemma alt_impl_validating_projection_prop:
+  valid_subsumes_constraint_prop ->
+  valid_message_is_protocol_in_composition_prop ->
+  validating_projection_prop.
+Proof.
+  intros Hcp Hpcp li [si omi] Hpv.
+  pose proof (Hcp' := Hcp li si omi Hpv).
+  pose proof (Hpcp' := Hpcp omi li si Hpv).
+  destruct Hcp' as [s [Hs [Hsi Hconstraint]]].
+  (*clear Hpv.*)
+  unfold vvalid. unfold valid. unfold machine. simpl.
+  (*exists (lift_to_composite_state IM i si).*)
+  exists s.
+  split.
+  { apply Hsi. }
+  unfold protocol_message_prop in Hpcp'.
+  destruct Hpcp' as [s' Hpp].
+  split; [assumption|].
+  
+  split.
+  { unfold option_protocol_message_prop.
+    exists s'.
+    apply Hpp.
+  }
+  unfold constrained_composite_valid.
+  split.
+  { unfold composite_valid. rewrite Hsi.
+    unfold protocol_valid in Hpv. destruct Hpv as [_ [_ Hvalid]]. apply Hvalid.
+  }
+  apply Hconstraint.
 Qed.
 
 (**
@@ -123,8 +176,7 @@ Qed.
 
 (**
 We say that component <<i>> is [validating_transitions] if any [valid]
-transition (from a reachable state) in component <<i>> can be "lifted" to
-a [protocol_transition] in <<X>>.
+transition in component <<i>> can be "lifted" to a [protocol_transition] in <<X>>.
 
 *)
 
@@ -152,21 +204,31 @@ is equivalent with the [validating_transitions] property.
 Lemma validating_projection_messages_transitions
     : validating_projection_prop -> validating_transitions.
 Proof.
-    intros Hvalidating si omi li Hpvi.
-    specialize (Hvalidating li (si, omi) Hpvi). clear Hpvi.
-    destruct Hvalidating as [s [Hsi [Hps [Hopm [Hvalid Hctr]]]]].
-    destruct (vtransition X (existT _ i li) (s, omi)) as (s', om') eqn:Heqt.
+    unfold validating_projection_prop. unfold validating_transitions.
+    unfold projection_valid. unfold protocol_transition.
+    simpl. intros.
+    specialize (H li (si, omi) H0). clear H0. simpl in H.
+    destruct H as [s [Hsi [Hps [Hopm [Hvalid Hctr]]]]].
+    remember (vtransition X (existT _ i li) (s, omi)) as t.
+    destruct t as [s' om'].
     exists s. exists s'. exists om'.
-    subst si.
-    repeat split; assumption.
+    symmetry in Hsi. subst si; simpl.
+    repeat split; try assumption.
+    unfold vtransition in Heqt.
+    simpl in Heqt.
+    remember (vtransition (IM i) li (s i, omi)) as t.
+    destruct t as [si' om''].
+    inversion Heqt; subst.
+    reflexivity.
 Qed.
 
 Lemma validating_transitions_messages
     : validating_transitions -> validating_projection_prop.
 Proof.
-    intros Hvalidating li (si,omi) Hpvi.
-    specialize (Hvalidating si omi li Hpvi). clear Hpvi.
-    destruct Hvalidating as [s [s' [om' [Hsi [Hvalid Htransition]]]]].
+    unfold validating_projection_prop. unfold validating_transitions. intros.
+    destruct siomi as [si omi].
+    specialize (H si omi li H0); clear H0.
+    destruct H as [s [s' [om' [Hsi [Hvalid Htransition]]]]].
     symmetry in Hsi.
     exists s. split; assumption.
 Qed.
@@ -185,16 +247,14 @@ Section pre_loaded_with_all_messages_validating_proj.
         .
 
 (**
-We can show that <<Preloaded>> is included in <<Xi>> by applying the meta-lemma
-[VLSM_incl_finite_traces_characterization], and by induction on the length
-of a trace. The [validating_projection_prop]erty is used to translate
-[protocol_valid]ity for the preloaded machine into the [projection_valid]ity.
+We can show that <<Preloaded>> is included in <<Xi>> by applying the
+meta-lemma [basic_VLSM_incl], using the [validating_projection_prop]erty and
+Lemma [protocol_message_projection] to show that its conditions are fulfilled.
 *)
 
     Lemma pre_loaded_with_all_messages_validating_proj_incl
         : VLSM_incl PreLoaded Xi.
     Proof.
-        (* reduce inclusion to inclusion of finite traces. *)
         apply VLSM_incl_finite_traces_characterization.
         intros.
         split; [|apply H].
@@ -209,11 +269,10 @@ of a trace. The [validating_projection_prop]erty is used to translate
     Qed.
 
 (**
-Given that any projection is included in the [pre_loaded_with_all_messages_vlsm]
-of its component (Lemma [proj_pre_loaded_with_all_messages_incl]), we conclude
-that <<Preloaded>> and <<Xi>> are trace-equal.  This means that all the
-byzantine behavior of a validating component is exhibited by its corresponding
-projection.
+Given that any projection is included in the [pre_loaded_with_all_messages_vlsm] of its component
+(Lemma [proj_pre_loaded_with_all_messages_incl]), we conclude that <<Preloaded>> and <<Xi>> are
+trace-equal.  This means that all the byzantine behavior of a
+validating component is exhibited by its corresponding projection.
 *)
     Lemma pre_loaded_with_all_messages_validating_proj_eq
         : VLSM_eq PreLoaded Xi.
@@ -238,8 +297,8 @@ Context
 
 (**
 Let us fix a (regular) VLSM <<X>>. <<X>> is (self-)validating if every [valid]
-reachable [state] and <<message>> are [protocol_state] and [protocol_message]
-for that VLSM, respectively.
+[state] and <<message>> are [protocol_state] and [protocol_message] for that
+VLSM, respectively.
 *)
 
 Definition validating_vlsm_prop
@@ -250,9 +309,9 @@ Definition validating_vlsm_prop
 
 (**
 In the sequel we will show that a VLSM with the [validating_vlsm_prop]erty
-is trace-equal to its associated [pre_loaded_with_all_messages_vlsm], basically
-meaning (due to Lemma [byzantine_pre_loaded_with_all_messages]) that all traces
-with the [byzantine_trace_prop]erty associated to a validating VLSMs are also
+is trace-equal to its associated [pre_loaded_with_all_messages_vlsm], basically meaning that
+(due to Lemma [byzantine_pre_loaded_with_all_messages]) all traces with
+the [byzantine_trace_prop]erty associated to a validating VLSMs are also
 [protocol_trace]s for that VLSM, meaning that the VLSM cannot exhibit
 byzantine behavior.
 *)
@@ -264,11 +323,11 @@ Context
 
 (**
 Let <<PreLoaded>> be the [pre_loaded_with_all_messages_vlsm] associated to X.
-From Lemma [vlsm_incl_pre_loaded_with_all_messages_vlsm] we know that <<X>> is
-included in <<PreLoaded>>.
+From Lemma [vlsm_incl_pre_loaded_with_all_messages_vlsm] we know that <<X>> is included
+in <<PreLoaded>>.
 
 To prove the converse we use the [validating_vlsm_prop]erty to
-verify the conditions of meta-lemma [VLSM_incl_finite_traces_characterization].
+verify the conditions of meta-lemma [basic_VLSM_incl].
 *)
 
     Lemma pre_loaded_with_all_messages_validating_vlsm_incl
@@ -276,12 +335,10 @@ verify the conditions of meta-lemma [VLSM_incl_finite_traces_characterization].
     Proof.
         unfold validating_vlsm_prop  in Hvalidating.
         destruct X as [T [S M]]. simpl in *.
-        (* redcuction to inclusion of finite traces. *)
         apply VLSM_incl_finite_traces_characterization.
         intros.
         split; [|apply H].
         destruct H as [Htr Hs].
-        (* reverse induction on the length of a trace. *)
         induction tr using rev_ind.
         - constructor. apply initial_is_protocol. assumption.
         - apply finite_protocol_trace_from_app_iff in Htr.
@@ -293,7 +350,6 @@ verify the conditions of meta-lemma [VLSM_incl_finite_traces_characterization].
           apply first_transition_valid in Hx.
           destruct Hx as [Hvx Htx].
           split; [|assumption].
-          (* using the [validating_vlsm_prop]erty. *)
           revert Hvx.
           apply Hvalidating.
     Qed.
