VLSM/ELMO.v
@@ -1,0 +1,2926 @@
+From Coq Require Import ssreflect ssrfun ssrbool.
+
+Require Import
+  List Coq.Vectors.Fin
+  Arith.Compare_dec Lia
+  Program Reals Lra ListSet Nat
+  Coq.Logic.FinFun
+  .
+Import ListNotations.
+From CasperCBC
+  Require Import
+    Preamble
+    Lib.Measurable
+    Lib.ListExtras
+    VLSM.Common
+    VLSM.Composition
+    VLSM.Validating
+    VLSM.Equivocation
+    .
+
+Require Import List.
+    
+Inductive Label := Receive | Send.
+
+Inductive Prestate : Type :=
+| Cprestate: list Observation -> Prestate
+with
+Observation : Type :=
+| Cobservation: Label -> Premessage -> nat -> Observation
+with
+Premessage : Type :=
+| Cpremessage: Prestate -> nat -> Premessage
+.
+
+Section induction_principle.
+  Context
+    (Pps : Prestate -> Prop)
+    (Plo : list Observation -> Prop)
+    (Pob : Observation -> Prop)
+    (Ppm : Premessage -> Prop)
+    (Hps : forall (l : list Observation), Plo l -> Pps (Cprestate l))
+    (Hlonil : Plo nil)
+    (Hlocons : forall (a : Observation) (l : list Observation),
+        Pob a ->
+        Plo l ->
+        Plo (a::l)
+    )
+    (Hob : forall (l : Label) (p : Premessage) (n : nat),
+        Ppm p ->
+        Pob (Cobservation l p n))
+    (Hpm : forall (p : Prestate) (n : nat),
+        Pps p ->
+        Ppm (Cpremessage p n))
+  .
+
+  Fixpoint
+    Prestate_mut_ind (p : Prestate) : Pps p :=
+    let ListObservation_mut_ind := (fix ListObservation_mut_ind (lo : list Observation) : Plo lo :=
+    match lo as lo0 return (Plo lo0) with
+    | [] => Hlonil
+    | y::lo0 => Hlocons y lo0 (Observation_mut_ind y) (ListObservation_mut_ind lo0)
+    end) in
+    match p as p0 return (Pps p0) with
+    | Cprestate l => Hps l (ListObservation_mut_ind l)
+    end
+  with
+  Observation_mut_ind (o : Observation) : Pob o :=
+    match o as o0 return (Pob o0) with
+    | Cobservation l p n => Hob l p n (Premessage_mut_ind p)
+    end
+  with
+  Premessage_mut_ind (p : Premessage) : Ppm p :=
+    match p as p0 return (Ppm p0) with
+    | Cpremessage p0 n => Hpm p0 n (Prestate_mut_ind p0)
+    end
+  .
+  
+End induction_principle.
+
+
+Fixpoint
+  Prestate_weight (p : Prestate) : nat :=
+  let ListObservation_weight := (fix ListObservation_weight (lo : list Observation) : nat :=
+                                    match lo as lo0 return nat with
+                                    | [] => 0
+                                    | y::lo0 => S ((Observation_weight y) + (ListObservation_weight lo0))
+                                    end) in
+  match p as p0 return nat with
+  | Cprestate l => 1 + (ListObservation_weight l)
+  end
+with
+Observation_weight (o : Observation) : nat :=
+  match o as o0 return nat with
+  | Cobservation l p n => 1 + (Premessage_weight p)
+  end
+with
+Premessage_weight (p : Premessage) : nat :=
+  match p as p0 return nat with
+  | Cpremessage p0 n => 1 + (Prestate_weight p0)
+  end
+.
+
+Definition ListObservation_weight := (fix ListObservation_weight (lo : list Observation) : nat :=
+                                    match lo as lo0 return nat with
+                                    | [] => 0
+                                    | y::lo0 => S ((Observation_weight y) + (ListObservation_weight lo0))
+                                    end).
+
+Instance Label_eqdec : EqDecision Label.
+Proof.
+  intros l1 l2.
+  unfold Decision.
+  decide equality.
+Qed.
+
+ 
+
+Lemma Prestate_eqdec : forall (s1 s2 : Prestate), {s1 = s2} + {s1 <> s2}
+with  Observation_eqdec : forall (o1 o2 : Observation), {o1 = o2} + {o1 <> o2}
+with  Premessage_eqdec : forall (m1 m2 : Premessage), {m1 = m2} + {m1 <> m2}.
+Proof.
+  decide equality. decide equality. decide equality. decide equality.
+  decide equality. decide equality. decide equality.
+Qed.
+
+Instance Prestate_eqdec' : EqDecision Prestate.
+Proof.
+  intros x y.
+  apply Prestate_eqdec.
+Qed.
+
+Instance Observation_eqdec' : EqDecision Observation.
+Proof.
+  intros x y.
+  apply Observation_eqdec.
+Qed.
+
+Instance Premessage_eqdec' : EqDecision Premessage.
+Proof.
+  intros x y.
+  apply Premessage_eqdec.
+Qed.
+
+Definition dummy_prestate := Cprestate [].
+Definition dummy_premessage := Cpremessage dummy_prestate 0.
+Definition dummy_observation := Cobservation Receive dummy_premessage 0.
+
+
+Definition observationsOf (prs : Prestate) : list Observation :=
+  match prs with
+  | Cprestate l => l
+  end.
+
+Definition labelOf (ob : Observation) : Label :=
+  match ob with
+  | Cobservation lbl _ _ => lbl
+  end.
+
+Definition messageOf (ob : Observation) : Premessage :=
+  match ob with
+  | Cobservation _ msg _ => msg
+  end.
+
+Definition witnessOf (ob : Observation) : nat :=
+  match ob with
+  | Cobservation _ _ w => w
+  end.
+
+Definition isWitnessedBy (component : nat) (ob : Observation) : bool :=
+  bool_decide (witnessOf ob = component).
+
+Definition isReceive (ob : Observation) : bool :=
+  match ob with
+  | Cobservation Receive _ _ => true
+  | _ => false
+  end.
+
+Definition isSend (ob : Observation) : bool :=
+  match ob with
+  | Cobservation Send _ _ => true
+  | _ => false
+  end.
+
+Definition stateOf (m : Premessage) : Prestate :=
+  match m with
+  | Cpremessage s _ => s
+  end.
+
+Definition authorOf (m : Premessage) : nat :=
+  match m with
+  | Cpremessage _ a => a
+  end.
+
+
+Instance elmo_type : VLSM_type Premessage :=
+  {| state := Prestate;
+     Common.label := Label;
+  |}.
+
+Definition elmo_state : Type := @state Premessage elmo_type.
+
+Definition elmo_initial_state_prop (ps : elmo_state) : Prop :=
+  observationsOf ps = [].
+
+Definition elmo_initial_state
+  := sig elmo_initial_state_prop.
+
+Definition elmo_s0 : elmo_initial_state.
+Proof.
+  unfold elmo_initial_state.
+  exists (Cprestate []).
+  unfold elmo_initial_state_prop.
+  reflexivity.
+Defined.
+
+Definition elmo_m0 : Premessage := Cpremessage (Cprestate []) 0.
+
+Definition elmo_sig : VLSM_sign elmo_type :=
+  {| initial_state_prop := elmo_initial_state_prop
+     ; s0 := elmo_s0
+     ; initial_message_prop := (fun x => False)
+     ; m0 := elmo_m0
+     ; l0 := Receive
+     ;
+  |}.
+
+
+(* Check that every message received or sent in m has been received in the prefix by the component *)
+Definition fullNode (m : Premessage) (prefix: list Observation) (component: nat) : bool :=
+  fold_right andb true
+             (map (fun (ob2 : Observation) =>
+                     if (decide (authorOf (messageOf ob2) = component)) then
+                       bool_decide (In (Cobservation Send (messageOf ob2) component) prefix)
+                     else
+                       bool_decide (In (Cobservation Receive (messageOf ob2) component) prefix)
+                  )
+                  (observationsOf (stateOf m))
+             ).
+
+
+Definition nth_update {A : Type} (l : list A) (idx : nat) (v : A) : list A :=
+  firstn idx l ++ cons v (skipn (S idx) l).
+
+Program Definition update
+           (m : Premessage)
+           (component : nat)
+           (weights : list pos_R)
+           (otreshold : option R)
+           (curState : list Prestate)
+           (curEq : set nat)
+  : bool * (list Prestate) * (set nat) :=
+  let p := stateOf m in
+  let a := authorOf m in
+  let lp := length (observationsOf p) in
+  let ca := nth a curState dummy_prestate in
+  let la := length (observationsOf (ca)) in
+  if andb (la <=? lp)
+          (bool_decide ((firstn la (observationsOf p))=(observationsOf ca))) then
+    (true,
+     nth_update curState a (Cprestate (observationsOf p ++ [Cobservation Send m a])),
+     curEq)
+  else
+    if andb (S lp <=? la)
+            (andb
+               (bool_decide ((firstn lp (observationsOf ca))=(observationsOf p)))
+               (bool_decide ((nth lp (observationsOf ca) dummy_observation)=(Cobservation Send m a)))) then
+      (true, curState, curEq)
+    else
+      let newEq := curEq in
+      match otreshold with
+      | Some treshold =>
+        if (Rlt_dec (@sum_weights _ (Build_Measurable _ (fun idx => nth idx weights (exist _ 1%R _))) newEq) treshold) then
+          (false, curState, curEq)
+        else
+          (true, curState, newEq)
+      | None => (true, curState, newEq)
+      end.
+Next Obligation.
+   lra.
+Defined.
+
+
+Definition isProtocol_step
+           (component : nat) (weights : list pos_R) (otreshold : option R) (observations : list Observation)
+           (args : bool * nat * list Prestate * set nat) (ob : Observation)
+  : bool * nat * list Prestate * set nat
+  :=
+    let: (result, i,  curState, curEq) := args in
+    match result with
+    | false => args
+    | true =>
+      let l := labelOf ob in
+      let m := messageOf ob in
+      let p := stateOf m in
+      let a := authorOf m in
+      let w := witnessOf ob in
+      let prefix := firstn i observations in
+      let i := S i in
+      (* w <> component *)
+      if negb (bool_decide (w=component)) then
+        (false, i, curState, curEq)
+      else (* w = component *)
+        if bool_decide (a=component) then
+          match l with
+          | Send =>
+            let result := bool_decide (observationsOf p = prefix) in
+            (result, i, curState, curEq)
+          | Receive =>
+            let result := bool_decide (In (Cobservation Send m component) prefix) in
+            (result, i, curState, curEq)
+          end
+        else
+          (* a <> component *)
+          match l with
+          | Send =>
+            let result := false in
+            (result, i, curState, curEq)
+          | Receive =>
+            if negb (fullNode m prefix component) then
+              let result := false in
+              (result, i, curState, curEq)
+            else
+              let: (result, curState, curEq) := update m component weights otreshold curState curEq in
+              (result, i, curState, curEq)
+          end 
+    end.
+
+Definition isProtocol
+           (prestate : Prestate)
+           (component : nat)
+           (weights : list pos_R)
+           (otreshold: option R) : bool
+  :=
+    let initialState := map (fun x => Cprestate nil) weights in
+    let initialEq := @nil nat in
+    let result := (fold_left (isProtocol_step component weights otreshold (observationsOf prestate)) (observationsOf prestate) (true, 0, initialState, initialEq )) in
+    fst (fst (fst result)).
+
+Definition elmo_valid
+           (addresses : list nat)
+           (component : nat)
+           (weights : list pos_R)
+           (otreshold : option R)
+           (label : Label)
+           (bsom : Prestate * option Premessage)
+  : bool :=
+  let: (state, message) := bsom in
+  match label,message with
+  | Send, None => true
+  | Send, Some _ => false
+  | Receive, None => false
+  | Receive, Some m =>
+    bool_decide (List.In (authorOf m) addresses) &&
+    fullNode m (observationsOf state) component &&
+    (if (decide (authorOf m = component)) then
+      bool_decide (List.In (Cobservation Send m component) (observationsOf state))
+    else
+      true
+    ) &&
+    isProtocol (stateOf m) (authorOf m) weights otreshold
+  end.
+
+Definition elmo_transition
+           (component : nat)
+           (weights : list pos_R)
+           (otreshold : option R)
+           (label : Common.label)
+           (bsom : Prestate * option Premessage)
+  : Prestate * option Premessage
+  :=
+    let: (state, message) := bsom in
+    match label, message with
+    | Send, Some _ => (state, None)
+    | Send, None
+      => let m := Cpremessage state component in
+         let ob := Cobservation Send m component in
+         let s := Cprestate (observationsOf state ++ [ob]) in
+         (s, Some m)
+    | Receive, None
+      => (state, None)
+    | Receive, Some msg
+      => let ob := Cobservation Receive msg component in
+         let s := Cprestate (observationsOf state ++ [ob]) in
+         (s, None)
+    end.
+
+Definition elmo_vlsm_machine (addresses : list nat)
+           (component : nat) (weights : list pos_R) (otreshold : option R)
+  : @VLSM_class Premessage elmo_type elmo_sig
+  :=
+    {| valid := elmo_valid addresses component weights otreshold
+       ; transition := elmo_transition component weights otreshold
+    |}.
+
+
+Section capabilities.
+  Context
+    (addresses : list nat)
+    (component : nat)
+    (weights : list pos_R)
+    (otreshold : option R)
+    (vlsm := mk_vlsm (elmo_vlsm_machine addresses component weights otreshold))
+  .
+
+  Check (field_selector input).
+  Check oracle_stepwise_props.
+
+  Definition elmo_has_been_received_oracle (s : Prestate) (m : Premessage) : Prop :=
+    List.In m (map messageOf (filter isReceive (filter (isWitnessedBy component) (observationsOf s)))).
+
+  Definition elmo_has_been_sent_oracle (s : Prestate) (m : Premessage) : Prop :=
+    List.In m (map messageOf (filter isSend (filter (isWitnessedBy component) (observationsOf s)))).
+
+  Lemma elmo_has_been_received_oracle_dec : RelDecision elmo_has_been_received_oracle.
+  Proof.
+    intros x y.
+    apply list_in_dec.
+  Qed.
+
+  Lemma elmo_has_been_sent_oracle_dec : RelDecision elmo_has_been_sent_oracle.
+  Proof.
+    intros x y.
+    apply list_in_dec.
+  Qed.
+
+  
+  Lemma elmo_has_been_received_oracle_no_inits:
+    forall (s : vstate vlsm),
+      initial_state_prop (VLSM_sign := sign vlsm) s ->
+      forall m, ~elmo_has_been_received_oracle s m.
+  Proof.
+    intros s Hinitial m Hcontra.
+    simpl in Hinitial. unfold elmo_initial_state_prop in Hinitial.
+    unfold elmo_has_been_received_oracle in Hcontra. rewrite Hinitial in Hcontra.
+    simpl in Hcontra.
+    exact Hcontra.
+  Qed.
+
+
+  Lemma elmo_has_been_received_oracle_step_update:
+    forall l s im s' om,      
+      protocol_transition (pre_loaded_with_all_messages_vlsm vlsm) l (s,im) (s',om) ->
+      forall msg, elmo_has_been_received_oracle s' msg <->
+                  ((field_selector input) msg {|l:=l; input:=im; destination:=s'; output:=om|}
+                   \/ elmo_has_been_received_oracle s msg).
+  Proof.
+    intros l s im s' om Hpt msg.
+    simpl.
+
+    destruct Hpt as [Hvalid Htransition].
+    simpl in Htransition.
+    unfold vtransition in Htransition. simpl in Htransition.
+    
+    unfold elmo_has_been_received_oracle.
+    destruct l, im; inversion Htransition; subst; clear Htransition; simpl.
+    - rewrite filter_app.
+      rewrite filter_app.
+      rewrite map_app.
+      rewrite in_app_iff.
+      simpl. unfold isWitnessedBy. simpl.
+      destruct (bool_decide (component = component)) eqn:Heq.
+      2: { apply bool_decide_eq_false in Heq. contradiction. }
+      clear Heq.
+      simpl.
+      split.
+      + intros [H|H].
+        * right. exact H.
+        * left. destruct H as [H|H].
+          ** congruence.
+          ** inversion H.
+      + intros [H|H].
+        * inversion H; subst.
+          right. left. reflexivity.
+        * left. exact H.
+    - split; intros H.
+      + right. exact H.
+      + destruct H.
+        * inversion H.
+        * exact H.
+    - split; intros H.
+      + right. exact H.
+      + destruct H.
+        * inversion H; subst.
+          inversion Hvalid.
+          destruct H1.
+          simpl in H2. unfold vvalid in H2. simpl in H2. inversion H2.
+        * exact H.
+    - rewrite filter_app.
+      rewrite filter_app.
+      rewrite map_app.
+      rewrite in_app_iff.
+      simpl. unfold isWitnessedBy. simpl.
+      destruct (bool_decide (component = component)) eqn:Heq.
+      2: { apply bool_decide_eq_false in Heq. contradiction. }
+      clear Heq.
+      simpl.
+      split.
+      + intros [H|H].
+        * right. exact H.
+        * inversion H.
+      + intros [H|H].
+        * inversion H.
+        * left. exact H.
+  Qed.
+
+  Definition elmo_has_been_received_oracle_stepwise_props
+    : @oracle_stepwise_props _ vlsm (field_selector input) elmo_has_been_received_oracle
+    := {| oracle_no_inits := elmo_has_been_received_oracle_no_inits;
+          oracle_step_update := elmo_has_been_received_oracle_step_update;
+       |}
+  .
+
+
+  Lemma elmo_has_been_sent_oracle_no_inits:
+    forall (s : vstate vlsm),
+      initial_state_prop (VLSM_sign := sign vlsm) s ->
+      forall m, ~elmo_has_been_sent_oracle s m.
+  Proof.
+    intros s Hinitial m Hcontra.
+    simpl in Hinitial. unfold elmo_initial_state_prop in Hinitial.
+    unfold elmo_has_been_sent_oracle in Hcontra. rewrite Hinitial in Hcontra.
+    simpl in Hcontra.
+    exact Hcontra.
+  Qed.
+
+
+  Lemma elmo_has_been_sent_oracle_step_update:
+    forall l s im s' om,      
+      protocol_transition (pre_loaded_with_all_messages_vlsm vlsm) l (s,im) (s',om) ->
+      forall msg, elmo_has_been_sent_oracle s' msg <->
+                  ((field_selector output) msg {|l:=l; input:=im; destination:=s'; output:=om|}
+                   \/ elmo_has_been_sent_oracle s msg).
+  Proof.
+    intros l s im s' om Hpt msg.
+    simpl.
+
+    destruct Hpt as [Hvalid Htransition].
+    simpl in Htransition.
+    unfold vtransition in Htransition. simpl in Htransition.
+    
+    unfold elmo_has_been_sent_oracle.
+    destruct l, im; inversion Htransition; subst; clear Htransition; simpl.
+    - rewrite filter_app.
+      rewrite filter_app.
+      rewrite map_app.
+      rewrite in_app_iff.
+      simpl. unfold isWitnessedBy. simpl.
+      destruct (bool_decide (component = component)) eqn:Heq.
+      2: { apply bool_decide_eq_false in Heq. contradiction. }
+      clear Heq.
+      simpl.
+      split.
+      + intros [H|H].
+        * right. exact H.
+        * inversion H.
+      + intros [H|H].
+        * inversion H.
+        * left. exact H.
+    - split; intros H.
+      + right. exact H.
+      + destruct H.
+        * inversion H.
+        * exact H.
+    - split; intros H.
+      + right. exact H.
+      + destruct H.
+        * inversion H; subst.
+        * exact H.
+    - rewrite filter_app.
+      rewrite filter_app.
+      rewrite map_app.
+      rewrite in_app_iff.
+      simpl. unfold isWitnessedBy. simpl.
+      destruct (bool_decide (component = component)) eqn:Heq.
+      2: { apply bool_decide_eq_false in Heq. contradiction. }
+      clear Heq.
+      simpl.
+      split.
+      + intros [H|H].
+        * right. exact H.
+        * destruct H.
+          ** left. congruence.
+          ** inversion H.
+      + intros [H|H].
+        * inversion H. right. left. reflexivity.
+        * left. exact H.
+  Qed.
+
+  Definition elmo_has_been_sent_oracle_stepwise_props
+    : @oracle_stepwise_props _ vlsm (field_selector output) elmo_has_been_sent_oracle
+    := {| oracle_no_inits := elmo_has_been_sent_oracle_no_inits;
+          oracle_step_update := elmo_has_been_sent_oracle_step_update;
+       |}
+  .
+
+  Instance elmo_has_been_sent_capability : has_been_sent_capability vlsm.
+  Proof.
+    eapply has_been_sent_capability_from_stepwise.
+    2: apply elmo_has_been_sent_oracle_stepwise_props.
+    apply elmo_has_been_sent_oracle_dec.
+  Defined.
+
+  Instance elmo_has_been_received_capability : has_been_received_capability vlsm.
+  Proof.
+    eapply has_been_received_capability_from_stepwise.
+    2: apply elmo_has_been_received_oracle_stepwise_props.
+    apply elmo_has_been_received_oracle_dec.
+  Defined.
+  
+End capabilities.
+
+Lemma Observation_in_list_weight ob l:
+  List.In ob l ->
+  Observation_weight ob < ListObservation_weight l.
+Proof.
+  intros H.
+  induction l.
+  + inversion H.
+  + simpl in H.
+    simpl.
+    destruct H as [H|H].
+    * subst. lia.
+    * specialize (IHl H). lia.
+Qed.
+
+
+Lemma Observation_nested_weight ob1 ob2:
+  List.In ob1 (observationsOf (stateOf (messageOf ob2))) ->
+  Observation_weight ob1 < Observation_weight ob2.
+Proof.
+  destruct ob2. destruct p. destruct p. simpl.
+  fold (ListObservation_weight l0).
+  intros H.
+  pose proof (H' := Observation_in_list_weight ob1 l0 H).
+  lia.
+Qed.
+
+
+Lemma Observation_nested_neq ob1 ob2:
+  List.In ob1 (observationsOf (stateOf (messageOf ob2))) ->
+  ob1 <> ob2.
+Proof.
+  intros H.
+  pose proof (H' := Observation_nested_weight ob1 ob2 H).
+  assert (Observation_weight ob1 <> Observation_weight ob2).
+  { lia. }
+  congruence.
+Qed.
+
+(* Observations of send messages contain all previous messages *)
+Definition ob_sent_contains_previous_prop l : Prop :=
+  forall (i : nat),
+    i < length l ->
+    labelOf (nth i l dummy_observation) = Send ->
+    forall (j : nat),
+      j < i ->
+      List.In
+        (nth j l dummy_observation)
+        (observationsOf (stateOf (messageOf (nth i l dummy_observation))))
+
+.
+
+
+Lemma ob_sent_contains_previous_prop_tail x xs:
+  ob_sent_contains_previous_prop (x :: xs) ->
+  ob_sent_contains_previous_prop xs.
+Proof.
+  unfold ob_sent_contains_previous_prop.
+  intros H.
+  intros i Hi Hsend j Hj.
+  simpl in H.
+  assert (Hi': S i < S (length xs)).
+  { lia. }
+  specialize (H (S i) Hi'). clear Hi'.
+  simpl in H.
+  assert (Hj': S j < S i).
+  { lia. }
+  specialize (H Hsend (S j) Hj'). clear Hj'.
+  simpl in H.
+  exact H.
+Qed.
+
+  
+
+Lemma ob_sent_contains_previous_prop_app l1 l2:
+  ob_sent_contains_previous_prop (l1 ++ l2) ->
+  ob_sent_contains_previous_prop l1 /\ ob_sent_contains_previous_prop l2.
+Proof.
+  intros H.
+  induction l1.
+  - simpl in H. split.
+    + unfold ob_sent_contains_previous_prop. intros i Hi. simpl in Hi. inversion Hi.
+    + exact H.
+  - simpl in H.
+    pose proof (Htail:= ob_sent_contains_previous_prop_tail _ _ H).
+    specialize (IHl1 Htail).
+    destruct IHl1 as [IHl11 IHl12].
+    split.
+    2: { exact IHl12. }
+    intros i Hi Hsend j Hj.
+    specialize (H i).
+    simpl in *.
+    rewrite app_length in H.
+    assert (Hi': i < S (length l1 + length l2)).
+    { lia. }
+    specialize (H Hi'). clear Hi'.
+    destruct i.
+    + specialize (H Hsend j Hj). destruct j.
+      * exact H.
+      * lia.
+    + rewrite app_nth1 in H.
+      { lia. }
+      specialize (H Hsend j Hj).
+      destruct j.
+      * exact H.
+      * rewrite app_nth1 in H.
+        { lia. }
+        exact H.
+Qed.
+
+Lemma ob_sent_contains_previous_prop_middle l1 a l2:
+  ob_sent_contains_previous_prop (l1 ++ a :: l2) ->
+  ob_sent_contains_previous_prop (l1 ++ l2).
+Proof.
+  intros H.
+  induction l1.
+  - simpl in *.
+    eapply ob_sent_contains_previous_prop_tail.
+    apply H.
+  - simpl in *.
+    specialize (IHl1 (ob_sent_contains_previous_prop_tail _ _ H)).
+    intros i Hi Hsend j Hj.
+    destruct j.
+    + (* j = 0 -> use H *)
+      clear IHl1.
+      destruct i.
+      { lia. }
+      clear Hj.
+      simpl in *.
+      rewrite app_length in Hi.
+      (* I need to case split on whether i < length l1 or not *)
+      destruct (dec_lt i (length l1)).
+      * rewrite app_nth1.
+        { apply H0. }        
+        specialize (H (S i)).
+        simpl in H.
+        assert (Htmp: (S i) < S (length (l1 ++ a :: l2))).
+        { rewrite app_length. simpl. lia. }
+        specialize (H Htmp). clear Htmp.
+        rewrite app_nth1 in H.
+        { apply H0. }
+        rewrite app_nth1 in Hsend.
+        { apply H0. }
+        specialize (H Hsend). clear Hsend.
+        specialize (H 0).
+        assert (Htmp: 0 < S i).
+        { lia. }
+        specialize (H Htmp). clear Htmp.
+        simpl in H. exact H.
+      * rewrite app_nth2.
+        { lia. }
+        rewrite app_nth2 in Hsend.
+        { lia. }
+        specialize (H (S (S i))).
+        simpl in H.
+        rewrite app_nth2 in H.
+        { lia. }
+        assert (Htmp: (S i) - (length l1) = S (i - (length l1))).
+        { lia. }
+        rewrite Htmp in H. clear Htmp.
+        simpl in H.
+        assert (Htmp: S (S i) < S (length (l1 ++ a :: l2))).
+        { rewrite app_length. simpl. lia. }
+        specialize (H Htmp Hsend). clear Htmp.
+        specialize (H 0).
+        assert (Htmp: 0 < S (S i)).
+        { lia. }
+        specialize (H Htmp). clear Htmp.
+        simpl in H. exact H.
+        
+      
+    + (* j > 0 -> use IHl1 *)
+      clear H.
+      simpl. simpl in Hsend.
+      destruct i.
+      { lia. }
+      apply IHl1.
+      3: { lia. }
+      2: { exact Hsend. }
+      simpl in Hi. lia.
+Qed.
+
+(* We now prove that all the states of a single component satisfy [ob_sent_contains_previous_prop].
+   We start with an initial state *)
+
+Lemma ob_sent_contains_previous_prop_initial : ob_sent_contains_previous_prop [].
+Proof.
+  intros i Hi Hx j Hj.
+  simpl in Hi.
+  inversion Hi.
+Qed.
+
+(* And prove that the transition function preserves this property. *)
+Lemma ob_sent_contains_previous_prop_step
+      (addresses : list nat)
+      (component : nat)
+      (weights : list pos_R)
+      (otreshold : option R)
+      (label : Label)
+      (bsom : Prestate * option Premessage) :
+  ob_sent_contains_previous_prop (observationsOf (fst bsom)) ->
+  elmo_valid addresses component weights otreshold label bsom ->
+  ob_sent_contains_previous_prop (observationsOf (fst (elmo_transition component weights otreshold label bsom))).
+Proof.
+  destruct bsom as [bs om].
+  intros Hinit Hvalid.
+  simpl. simpl in Hinit.
+  destruct label.
+  - (* Receive *)
+    destruct om.
+    + simpl.
+      unfold ob_sent_contains_previous_prop.
+      simpl.
+      intros i Hi Hsend j Hj.
+      destruct (decide (i = length (observationsOf bs))).
+      * subst i.
+        rewrite nth_middle in Hsend.
+        simpl in Hsend.
+        inversion Hsend.
+      * rewrite app_length in Hi. simpl in Hi.
+        assert (Hi2: i < length (observationsOf bs)).
+        { lia. }
+        clear Hi. clear n.
+        unfold ob_sent_contains_previous_prop in Hinit.
+        rewrite app_nth1.
+        { lia. }
+        rewrite app_nth1.
+        { assumption. }
+        rewrite app_nth1 in Hsend.
+        { apply Hi2. }
+        apply Hinit.
+        { apply Hi2. }
+        { apply Hsend. }
+        { apply Hj. }
+    + simpl. exact Hinit.
+  - destruct om; simpl.
+    + apply Hinit.
+    + unfold ob_sent_contains_previous_prop. simpl.
+      intros i Hi Hsend j Hj.
+      destruct (decide (i = length (observationsOf bs))).
+      * subst i.
+        clear Hsend.
+        rewrite app_nth1.
+        { apply Hj. }
+        rewrite nth_middle.
+        simpl.
+        apply nth_In.
+        apply Hj.
+      * rewrite app_length in Hi. simpl in Hi.
+        assert (Hi2: i < length (observationsOf bs)).
+        { lia. }
+        clear Hi. clear n.
+        unfold ob_sent_contains_previous_prop in Hinit.
+        rewrite app_nth1.
+        { lia. }
+        rewrite app_nth1.
+        { assumption. }
+        rewrite app_nth1 in Hsend.
+        { apply Hi2. }
+        apply Hinit.
+        { apply Hi2. }
+        { apply Hsend. }
+        { apply Hj. }
+Qed.
+
+(* If we have an observation of a received message, the message is not sent later
+  (assuming [ob_sent_contains_previous_prop]).
+ *)
+
+Lemma ob_sent_contains_previous_prop_impl_received_is_not_sent_later component m l2:
+  ob_sent_contains_previous_prop ((Cobservation Receive m component) :: l2) ->
+  ~List.In (Cobservation Send m component) l2.
+Proof.
+  intros H.
+  induction l2.
+  - simpl. intros [].
+  - simpl. intros Hcontra.
+    destruct Hcontra.
+    + subst.
+      unfold ob_sent_contains_previous_prop in H.
+      specialize (H 1).
+      simpl in H.
+      assert (H1 : 1 < S (S (length l2))).
+      { lia. }
+      specialize (H H1 (eq_refl _) 0).
+      assert (H0 : 0 < 1).
+      { lia. }
+      specialize (H H0). clear H0 H1.
+      simpl in H.
+      remember (Cobservation Receive m component) as ob1.
+      assert (Hm: m = messageOf ob1).
+      { subst. reflexivity. }
+      rewrite Hm in H.
+      pose proof (Observation_nested_neq _ _ H).
+      contradiction.
+    + apply IHl2.
+      2: apply H0.
+      clear H0 IHl2.
+      assert (Heq1: Cobservation Receive m component :: a :: l2 = [Cobservation Receive m component] ++ a :: l2).
+      { reflexivity. }
+      rewrite Heq1 in H. clear Heq1.
+      assert (Heq2: Cobservation Receive m component :: l2 = [Cobservation Receive m component] ++ l2).
+      { reflexivity. }
+      rewrite Heq2. clear Heq2.
+      eapply ob_sent_contains_previous_prop_middle.
+      eexact H.
+Qed.
+
+
+(* Now we can prove the lemma saying that [isProtocol_step] ignores the rest
+   of the list after [x]. Specifically, if [isProtocol_step] is given the index [i],
+   it uses only the observations with lower or equal index.
+ *)
+Lemma isProtocol_step_in component weights treshold l1 l2 args x:
+  let: (result, i,  curState, curEq) := args in
+  i = length l1 ->
+  ob_sent_contains_previous_prop (l1 ++ x :: l2) ->
+  let step := isProtocol_step component weights treshold in
+  step (l1 ++ x :: l2) args x =
+  step (l1 ++ [x]) args x.
+Proof.
+  destruct args as [[[b i] curState] curEq].
+  intros Hi Hprev.
+  simpl.
+  unfold isProtocol_step.
+  destruct x. destruct p.
+  subst i.
+  induction l1.
+  - destruct l; destruct b; destruct p; simpl; try reflexivity;
+    destruct (bool_decide (n0 = component)) eqn:Heqn0;
+    destruct (bool_decide (n = component)) eqn:Heqn; simpl; try reflexivity.
+  - simpl in Hprev.
+    specialize (IHl1 (ob_sent_contains_previous_prop_tail _ _ Hprev)).
+    destruct b.
+    2: { reflexivity. }
+    destruct (bool_decide (witnessOf (Cobservation l (Cpremessage p n0) n) = component)); simpl.
+    2: { reflexivity. }
+    simpl in IHl1.
+    destruct (bool_decide (n0 = component)),l; simpl in *.
+    4: { reflexivity. }
+    + inversion IHl1. clear IHl1.
+      repeat (apply pair_equal_spec; split); try reflexivity.
+      apply bool_decide_iff.
+      split; intros [H|H].
+      * left. subst a. reflexivity.
+      * right.
+        rewrite firstn_app.
+        rewrite Nat.sub_diag.
+        simpl.
+        rewrite -app_nil_end.
+        rewrite firstn_app in H.
+        rewrite Nat.sub_diag in H.
+        simpl in H.
+        rewrite -app_nil_end in H.
+        exact H.
+      * left. subst a. reflexivity.
+      * right.
+        apply bool_decide_iff_iff in H0.
+        apply H0. apply H.
+    + repeat rewrite firstn_app.
+      repeat rewrite Nat.sub_diag.
+      reflexivity.
+    + repeat rewrite firstn_app.
+      repeat rewrite Nat.sub_diag.
+      simpl. simpl in IHl1.
+      repeat rewrite -app_nil_end.
+      reflexivity.
+Qed.
+
+(* But how do we know that the assumption [ob_sent_contains_previous_prop]
+   of [isProtocol_step_in] holds? Yes, it holds on all local states, because we
+   proved it is an invariant; however, [isProtocol_step] is called with a list of observations
+   from a state contained in a received message. About the received message we know only that
+   it satisfies [isProtocol]; therefore, we need to prove that [isProtocol] implies
+   [ob_sent_contains_previous_prop], which is what
+   the lemma [isProtocol_implies_ob_sent_contains_previous_prop] is about.
+   Before that we prove some helper results.
+ *)
+
+
+Lemma isProtocol_step_false component weights treshold l x n curState curEq:
+  isProtocol_step component weights treshold l (false, n, curState, curEq) x
+  = (false, n, curState, curEq).
+Proof.
+  reflexivity.
+Qed.
+
+Lemma isProtocol_step_fold_false component weights treshold l1 l2 n curState curEq:
+(fold_left (isProtocol_step component weights treshold l1) l2
+           (false, n, curState, curEq)).1.1.1 = false.
+Proof.
+  induction l2.
+  - reflexivity.
+  - simpl. apply IHl2.
+Qed.
+
+Lemma isProtocol_step_fold_result_true component weights treshold l1 l2 b n curState curEq:
+  (fold_left (isProtocol_step component weights treshold l1) l2
+             (b, n, curState, curEq)).1.1.1 = true ->
+  b = true
+.
+Proof.
+  intros H.
+  destruct b.
+  - reflexivity.
+  - pose proof (H' := isProtocol_step_fold_false component weights treshold l1 l2 n curState curEq).
+    rewrite H' in H.
+    exact H.
+Qed.
+
+Lemma isProtocol_step_result_true component weights treshold l args ob:
+  (isProtocol_step component weights treshold l args ob).1.1.1 = true ->
+  args.1.1.1 = true.
+Proof.
+  intros H. simpl in H.
+  destruct args as [[[b n] curState] curEq].
+  destruct b.
+  { reflexivity. }
+  simpl in H. exact H.
+Qed.
+
+Lemma isProtocol_step_fold_result_true_idx component weights treshold l1 l2 args:
+  let: (_, n, _, _) := args in
+  let: (b', n', _, _) := (fold_left (isProtocol_step component weights treshold l1) l2 args) in
+  b' = true -> n' = n + length l2.
+Proof.
+  destruct args as [[[b n] curState] curEq].
+  move: b n curState curEq.
+  induction l2; intros b n curState curEq.
+  - simpl. auto.
+  - cbn [fold_left].
+    remember (isProtocol_step component weights treshold l1) as step.
+    remember (step (b,n,curState,curEq) a) as args1.
+    destruct args1 as [[[b1 n1] curState1] curEq1].
+    remember (fold_left step l2 (b1, n1, curState1, curEq1)) as result.
+    destruct result as [[[b' n'] curState'] curEq'].
+    intros Hb'. subst b'.
+    assert (Hfltrue: (fold_left step l2 (b1, n1, curState1, curEq1)).1.1.1 = true).
+    { rewrite -Heqresult. reflexivity. }
+    rewrite Heqstep in Hfltrue.
+    apply isProtocol_step_fold_result_true in Hfltrue.
+    subst b1.
+    simpl.
+    specialize (IHl2 true n1 curState1 curEq1).
+    rewrite -Heqresult in IHl2.
+    specialize (IHl2 (eq_refl _)).
+    subst n'.
+
+    assert (Hb: b = true).
+    {
+      pose proof (H := isProtocol_step_result_true component weights treshold l1 (b, n, curState, curEq) a).
+      rewrite Heqstep in Heqargs1.
+      rewrite -Heqargs1 in H.
+      simpl in H.
+      specialize (H (eq_refl _)).
+      exact H.
+    }
+    subst b.
+
+    assert (n1 = S n).
+    { clear Heqresult curEq' curState'.
+      rewrite Heqstep in Heqargs1.
+      cbn [isProtocol_step] in Heqargs1.
+      destruct (bool_decide (witnessOf a = component)); simpl in Heqargs1.
+      2: { inversion Heqargs1. }
+      destruct (bool_decide (authorOf (messageOf a) = component)), (labelOf a);
+        simpl in Heqargs1.
+      4: { inversion Heqargs1. }
+      2: { inversion Heqargs1. subst. reflexivity. }
+      1: { inversion Heqargs1. subst. reflexivity. }
+      destruct (fullNode (messageOf a) (firstn n l1) component); simpl in Heqargs1.
+      2: { inversion Heqargs1. }
+      destruct (update (messageOf a) component weights treshold curState curEq).
+      destruct p.
+      inversion Heqargs1. subst. reflexivity.
+    }
+    lia.
+Qed.
+
+Lemma isProtocol_step_app component weights treshold l1 l2 ob idx curState curEq:
+  idx <= length l1 ->
+  isProtocol_step component weights treshold (l1 ++ l2)
+                  (true, idx, curState, curEq)
+                  ob
+  = isProtocol_step component weights treshold l1
+                    (true, idx, curState, curEq) ob.
+Proof.
+  intros Hidx.
+  unfold isProtocol_step.
+  repeat rewrite firstn_app.
+  assert (Hidx': idx - length l1 = 0).
+  { lia. }
+  repeat rewrite Hidx'.
+  rewrite app_nil_r.
+  reflexivity.
+Qed.
+
+Lemma isProtocol_step_app_fold component weights otreshold l1 l2 l3 args:
+  let: (b, idx, curState, curEq) := args in
+  length l3 + idx <= length l1 ->
+  fold_left (isProtocol_step component weights otreshold (l1 ++ l2)) l3 args
+  = fold_left (isProtocol_step component weights otreshold l1) l3 args.
+Proof.
+  move: args.
+  induction l3; intros args.
+  - destruct args as [[[b idx] curState] curEq].
+    auto.
+  - destruct args as [[[b idx] curState] curEq].
+    intros Hlen.
+    simpl in Hlen.
+    cbn [ fold_left ].
+    remember (isProtocol_step component weights otreshold l1 (true, idx, curState, curEq) a) as stp.
+    destruct stp as [[[b' idx'] curState'] curEq'] eqn:Heqstp'.
+    assert (idx' = S idx).
+    { unfold isProtocol_step in Heqstp.
+      destruct (bool_decide (witnessOf a = component)); simpl in Heqstp.
+      2: { inversion Heqstp. subst. reflexivity. }
+      destruct (bool_decide (authorOf (messageOf a) = component)), (labelOf a);
+        simpl in Heqstp; inversion Heqstp; subst; try reflexivity.
+      clear H0.
+      destruct (fullNode (messageOf a) (firstn idx l1) component);
+        simpl in Heqstp; inversion Heqstp.
+      2: reflexivity.
+      destruct (update (messageOf a) component weights otreshold curState curEq).
+      destruct p.
+      inversion Heqstp. subst. reflexivity.
+    }
+    destruct b.
+    + rewrite isProtocol_step_app.
+      { lia. }
+
+      rewrite -Heqstp.
+      simpl in IHl3.
+      specialize (IHl3 stp).
+      rewrite Heqstp' in IHl3.
+      apply IHl3.
+      lia.
+    + repeat rewrite isProtocol_step_false.
+      remember (false, idx, curState, curEq) as args.
+      specialize (IHl3 args).
+      subst args. apply IHl3. lia.
+Qed.
+
+  
+Lemma isProtocol_last component weights otreshold l x:
+  isProtocol (Cprestate (l ++ [x])) component weights otreshold ->
+  isProtocol (Cprestate l) component weights otreshold.
+Proof.
+  unfold isProtocol.
+  simpl.
+  rewrite fold_left_app.
+  simpl.
+  intros H.
+  inversion H. clear H. rename H1 into H.
+  
+  remember (fold_left (isProtocol_step component weights otreshold (l ++ [x])) l
+            (true, 0, map (fun=> Cprestate []) weights, [])) as FL1.
+
+  pose proof (H' := isProtocol_step_result_true _ _ _ _ _ _ H).
+  remember (isProtocol_step component weights otreshold (l ++ [x]) FL1 x) as ARG2.
+  rewrite H.
+  subst ARG2. clear H.
+  pose proof (Htmp := isProtocol_step_app_fold component weights otreshold l [x] l
+                                               (true, 0, map (fun=> Cprestate []) weights, [])).
+  simpl in Htmp.
+  rewrite Htmp in HeqFL1.
+  { lia. }
+  rewrite -HeqFL1. rewrite H'. reflexivity.
+Qed.
+     
+
+Lemma isProtocol_implies_ob_sent_contains_previous_prop component weights otreshold l:
+  isProtocol (Cprestate l) component weights otreshold ->
+  ob_sent_contains_previous_prop l.
+Proof.
+  intros H.
+  induction l using rev_ind.
+  - unfold ob_sent_contains_previous_prop.
+    intros i Hi. simpl in Hi. inversion Hi.
+  - pose proof (isProtocol_last _ _ _ _ _ H).
+    specialize (IHl H0). clear H0.
+    unfold isProtocol in H.
+    rewrite fold_left_app in H.
+    simpl in H.
+    remember (fold_left (isProtocol_step component weights otreshold (l ++ [x])) l
+                        (true, 0, map (fun=> Cprestate []) weights, [])) as FL.
+    pose proof (HFLtrue := isProtocol_step_result_true _ _ _ _ _ _ H).
+    intros i Hi Hlbl j Hj.
+    rewrite app_length in Hi.
+    simpl in Hi.
+    destruct (decide(i = length l)).
+    2: { assert (i < length l).
+         { lia. }
+         rewrite app_nth1.
+         { lia. }
+         rewrite app_nth1.
+         { lia. }
+         rewrite app_nth1 in Hlbl.
+         { lia. }
+         apply IHl.
+         { lia. }
+         apply Hlbl.
+         exact Hj.
+    }
+    subst i.
+    rewrite app_nth1.
+    { exact Hj. }
+    rewrite nth_middle.
+    unfold isProtocol_step in H.
+    destruct FL as [[[tt i'] curState'] curEq'].
+    simpl in HFLtrue. subst tt.
+    destruct (bool_decide (witnessOf x = component)) eqn:Hwitness, (labelOf x) eqn:Hlabel; simpl in H.
+    4: { inversion H. }
+    3: { inversion H. }
+    { rewrite nth_middle in Hlbl. rewrite Hlabel in Hlbl. inversion Hlbl. }
+    destruct (bool_decide (authorOf (messageOf x) = component)) eqn:Hauthor; simpl in H.
+    2: { inversion H. }
+    clear Hlabel Hlbl.
+    destruct x. simpl in *.
+    destruct p. simpl in *.
+    destruct p. simpl in *.
+    apply bool_decide_eq_true in Hwitness. subst n.
+    apply bool_decide_eq_true in Hauthor. subst n0.
+    apply bool_decide_eq_true in H.
+    clear Hi.
+    rewrite H.
+    (* Now l1 is a prefix of l *)
+    (* First, i' = length l *)
+    pose proof (Hidx := isProtocol_step_fold_result_true_idx component weights otreshold).
+    specialize (Hidx (l ++ [Cobservation l0 (Cpremessage (Cprestate l1) component) component])).
+    specialize (Hidx l (true, 0, map (fun=> Cprestate []) weights, [])).
+    simpl in Hidx.
+    rewrite -HeqFL in Hidx.
+    specialize (Hidx (eq_refl _)).
+    subst i'.
+    rewrite firstn_app. rewrite Nat.sub_diag. simpl. rewrite app_nil_r. rewrite firstn_all.
+    apply nth_In. apply Hj.
+Qed.
+
+
+
+Lemma fold_isProtocol_step_app component weights otreshold l1 l2 b (*n*) s es:
+  ob_sent_contains_previous_prop (l1 ++ l2) ->
+  let FL := fold_left (isProtocol_step component weights otreshold (l1 ++ l2)) l1 (b, (*n*)0, s, es) in
+  FL.1.1.1 = true ->
+  FL = fold_left (isProtocol_step component weights otreshold l1) l1 (b, (*n*)0, s, es).
+Proof.
+  simpl.
+  generalize dependent l2.
+  generalize dependent b.
+  (*generalize dependent n.*)
+  generalize dependent s.
+  generalize dependent es.
+  (* TODO assume n <= length l1 *)
+  remember (length l1) as len.
+  assert (Hlen: length l1 <= len).
+  { lia. }
+  clear Heqlen.
+  revert Hlen.
+  generalize dependent l1.
+  induction len; intros l1 Hlen es s (*n*) b l2 Hoscp Htrue.
+  - destruct l1.
+    + reflexivity.
+    + simpl in Hlen. lia.
+  - destruct (null_or_exists_last l1).
+    { subst. reflexivity. }
+    destruct H as [l1' [x Hl1]].
+    remember (isProtocol_step component weights otreshold) as step.
+    remember (fold_left (step l1) l1 (b, (*n*)0, s, es)) as fl.
+    destruct fl as [[[b' n'] s'] es'].
+    rewrite Hl1. rewrite fold_left_app. simpl.
+    rewrite -app_assoc.
+
+    assert (Hlenl1': length l1' <= len).
+    { subst l1. rewrite app_length in Hlen. simpl in Hlen. lia. }
+
+    assert (Htrue': (fold_left (step (l1' ++ [x] ++ l2)) l1' (b, 0, s, es)).1.1.1 = true).
+    {
+      subst.
+      rewrite fold_left_app in Htrue. simpl in Htrue.
+      apply isProtocol_step_result_true in Htrue.
+      rewrite app_assoc. exact Htrue.
+    }
+    
+    rewrite IHlen.
+    { lia. }
+    { subst. rewrite app_assoc. exact Hoscp. }
+    { exact Htrue'. }
+    simpl.
+
+    remember (fold_left (step l1') l1' (b, (*n*)0, s, es)) as fl'.
+    destruct fl' as [[[b'' n''] s''] es''].
+    subst l1.
+    (*rewrite Hl1 in Heqfl.*)
+
+    rewrite fold_left_app in Heqfl. simpl in Heqfl.
+
+
+    assert (Htrue'': (fold_left (step (l1' ++ [x])) l1' (b, 0, s, es)).1.1.1 = true).
+    { subst.
+      rewrite app_assoc in Htrue'.
+      pose proof (Htmp := isProtocol_step_app_fold component weights otreshold (l1' ++ [x]) l2 l1' (b, 0, s, es)).
+      cbv beta iota in Htmp. rewrite Htmp in Htrue'.
+      { rewrite app_length. simpl. lia. }
+      exact Htrue'.
+    }
+    
+    
+    rewrite IHlen in Heqfl.
+    { lia. }
+    { exact (proj1 (ob_sent_contains_previous_prop_app _ _ Hoscp)). }
+    { exact Htrue''. }
+    
+    rewrite -Heqfl' in Heqfl.
+    rewrite Heqfl.
+    rewrite Heqstep.
+
+    (*
+    assert (Htrue''': (fold_left (step (l1' ++ [x] ++ l2)) l1' (b, 0, s, es)).1.1.1 = true).
+    { subst. *)
+
+    assert (Htrue''': (fold_left (step l1') l1' (b, 0, s, es)).1.1.1 = true).
+    { subst.
+      pose proof (Htmp := isProtocol_step_app_fold component weights otreshold l1' [x] l1' (b, 0, s, es)).
+      simpl in Htmp.
+      rewrite Htmp in Htrue''.
+      { lia. }
+      exact Htrue''.
+    }
+
+    assert (n'' = length l1').
+    { subst.
+      pose proof (Htmp := isProtocol_step_fold_result_true_idx component weights otreshold l1' l1' (b, 0, s, es)).
+      cbv beta iota in Htmp. rewrite -Heqfl' in Htmp. simpl in Htmp.
+      apply Htmp. clear Htmp.
+      rewrite -Heqfl' in Htrue'''.
+      simpl in Htrue'''.
+      exact Htrue'''.
+    }
+    subst n''.
+
+    pose proof (Hs := isProtocol_step_in component weights otreshold l1' l2 (b'', (length l1'), s'', es'') x).
+    cbv iota zeta beta in Hs.
+    specialize (Hs (eq_refl _)).
+    apply Hs.
+    rewrite -app_assoc in Hoscp.
+    simpl in Hoscp.
+    exact Hoscp.
+Qed.
+
+Lemma fullNode_appone (l obs : list Observation) (ob : Observation) (n component : nat) :
+  fullNode (Cpremessage (Cprestate (l ++ [ob])) n) obs component ->
+  fullNode (Cpremessage (Cprestate l) n) obs component.
+Proof.
+  intros H.
+  induction l using rev_ind.
+  - unfold fullNode. simpl. exact is_true_true.
+  - unfold fullNode. simpl.
+    unfold fullNode in H.
+    simpl in H.
+    rewrite map_app in H.
+    rewrite fold_right_app in H.
+    simpl in H.
+    destruct ob. simpl in H.
+    destruct (decide (authorOf p = component)); simpl in H.
+    {
+      destruct (bool_decide (In (Cobservation Send p component) obs)).
+      { simpl in H. exact H. }
+      simpl in H.
+      rewrite fold_right_andb_false in H. inversion H.
+    }
+    destruct (bool_decide (In (Cobservation Receive p component) obs)).
+    { simpl in H. exact H. }
+    { simpl in H. rewrite fold_right_andb_false in H. inversion H. }
+Qed.
+
+Lemma fullNode_dropMiddle (l1 l2 obs : list Observation) (ob : Observation) (n component : nat) :
+  fullNode (Cpremessage (Cprestate (l1 ++ (ob :: l2))) n) obs component ->
+  fullNode (Cpremessage (Cprestate (l1 ++ l2)) n) obs component.
+Proof.
+  intros H.
+  move: l1 H.
+  induction l2; intros l1 H.
+  - simpl. rewrite app_nil_r. eapply fullNode_appone. apply H.
+  - apply Forall_fold_right_bool. apply Forall_fold_right_bool in H.
+    simpl in H. simpl.
+    apply Forall_app in H. destruct H as [H1 H2].
+    apply Forall_app. split; [exact H1|]. clear H1.
+    inversion H2. subst. clear H2. exact H3.
+Qed.
+
+
+Lemma fullNode_last_receive_self (l obs : list Observation) (p : Prestate) (n n0 component : nat) :
+  fullNode (Cpremessage (Cprestate (l ++ [Cobservation Receive (Cpremessage p component) n0])) n) obs component = true ->
+  List.In (Cobservation Send (Cpremessage p component) component) obs.
+Proof.
+  intros Hfn.
+  induction l using rev_ind.
+  - unfold fullNode in Hfn.
+    simpl in Hfn.
+    destruct (decide (component = component)).
+    2: { contradiction. }
+    simpl in Hfn.
+    apply andb_prop in Hfn. destruct Hfn as [Hfn _].
+    apply bool_decide_eq_true_1 in Hfn.
+    exact Hfn.
+  - rewrite -app_assoc in Hfn. simpl in Hfn.
+    apply fullNode_dropMiddle in Hfn. auto.
+Qed.
+
+Lemma fullNode_last_receive_not_self (l obs : list Observation) (p : Prestate)
+      (n component1 component2 component3 : nat) :
+  component1 <> component2 ->
+  let ob := Cobservation Receive (Cpremessage p component2) component3 in
+  fullNode (Cpremessage (Cprestate (l ++ [ob])) n) obs component1 = true ->
+  List.In (Cobservation Receive (Cpremessage p component2) component1) obs.
+Proof.
+  intros Hneq ob Hfn.
+  induction l using rev_ind.
+  - unfold fullNode in Hfn. simpl in Hfn.
+    destruct (decide (component2 = component1)).
+    { subst. contradiction. }
+    simpl in Hfn.
+    apply andb_prop in Hfn. destruct Hfn as [Hfn _].
+    apply bool_decide_eq_true_1 in Hfn.
+    exact Hfn.
+  - rewrite -app_assoc in Hfn. simpl in Hfn.
+    apply fullNode_dropMiddle in Hfn. auto.
+Qed.
+
+Definition all_received_satisfy_isprotocol_prop {weights} {treshold} (obs : list Observation) : Prop :=
+  Forall (fun (ob : Observation) =>
+            if (isReceive ob) then
+              isProtocol (stateOf (messageOf ob)) (authorOf (messageOf ob)) weights treshold
+            else
+              true
+         ) obs.
+
+(*
+Lemma fullNode_length component obs m:
+  fullNode m obs component ->
+ *)
+
+Lemma Observation_list_weight_last l ob:
+  Observation_weight ob < ListObservation_weight (l ++ [ob]).
+Proof.
+  apply Observation_in_list_weight.
+  apply in_or_app.
+  right. simpl. left. reflexivity.
+Qed.
+
+(* m1 is a prefix of m2 *)
+Definition is_prefix_of (m1 m2 : Premessage) : Prop :=
+  let s1 := stateOf m1 in
+  let s2 := stateOf m2 in
+  observationsOf s1 = firstn (length (observationsOf s1)) (observationsOf s2).
+
+Lemma is_prefix_of_dec : RelDecision is_prefix_of.
+Proof.
+  intros m1 m2.
+  unfold is_prefix_of.
+  apply list_eq_dec.
+  apply Observation_eqdec.
+Qed.
+
+Definition equivocation_evidence (m1 m2 : Premessage) : Prop :=
+  authorOf m1 = authorOf m2 /\
+  ~ is_prefix_of m1 m2 /\
+  ~ is_prefix_of m2 m1.
+
+Instance equivocation_evidence_dec : RelDecision equivocation_evidence.
+Proof.
+  intros m1 m2.
+  unfold equivocation_evidence.
+  apply Decision_and.
+  { unfold Decision. decide equality. }
+  apply Decision_and; apply Decision_not; apply is_prefix_of_dec.
+Qed.
+
+(* `component` is equivocating and we have an evidence in the state `s` (of another component) *)
+Definition is_equivocator (component : nat) (s : Prestate) : bool :=
+  let obs := observationsOf s in
+  existsb
+    (fun ob1 =>
+       existsb
+         (fun ob2 =>
+            bool_decide (labelOf ob1 = Receive) &&
+            bool_decide (labelOf ob2 = Receive) &&
+            bool_decide (authorOf (messageOf ob1) = component) &&
+            bool_decide (authorOf (messageOf ob2) = component) &&
+            bool_decide (equivocation_evidence (messageOf ob1) (messageOf ob2))
+         )
+         obs
+    )
+    obs.
+
+Section composition.
+
+  Context
+    (weights : list pos_R)
+    (otreshold : option R)
+    (index : Type)
+    {i0 : Inhabited index}
+    {IndEqDec : EqDecision index}
+    (indices : list index)
+    (finite_index : Listing indices)
+    (indices_weights_eqlenght : length indices = length weights)
+  .
+
+  Definition addresses : list nat := seq 0 (length indices).
+
+  Definition index_to_component (idx : index) : nat :=
+    findInList idx indices.
+  
+  Definition component_to_index (component : nat) : index :=
+    nth component indices (@inhabitant _ i0).
+
+  Lemma index_to_component_to_index (idx : index) :
+    component_to_index (index_to_component idx) = idx.
+  Proof.
+    unfold component_to_index.
+    unfold index_to_component.
+    apply findInList_correct.
+    apply finite_index.
+  Qed.
+
+  Definition address_valid (a : nat) : Prop :=
+    a < length indices.
+
+  Instance address_valid_dec (a : nat) : Decision (address_valid a).
+  Proof.
+    unfold address_valid.
+    apply lt_dec.
+  Qed.
+  
+  Lemma component_to_index_to_component (a : nat) :
+    address_valid a ->
+    index_to_component (component_to_index a) = a.
+  Proof.
+    intros Hvalid.
+    unfold index_to_component.
+    unfold component_to_index.
+    apply findInList_nth.
+    { exact Hvalid. }
+    { apply finite_index. }
+  Qed.
+
+  
+  Definition IM' (i : index) := elmo_vlsm_machine addresses (index_to_component i) weights otreshold.
+  Definition IM (i : index) := mk_vlsm (IM' i).
+
+  (* `component` is equivocating and we have an evidence in some state
+     of the list `states` *)
+  Definition is_equivocator_states (states : list Prestate) (component : nat) : bool :=
+    let eq := map (is_equivocator component) states in
+    fold_right orb false eq.
+
+  Definition equivocators (states : list Prestate) : list nat :=
+    filter (is_equivocator_states states) (seq 0 (length indices)).
+  
+  Program Definition composition_constraint
+             (cl : composite_label IM)
+             (sm : composite_state IM * option Premessage) : Prop
+    := let cs := fst sm in
+       let om := snd sm in
+       match om with
+       | None => True
+       | Some m =>
+         let states := map cs indices in
+         let transitions := map (fun i => @transition _ _ _ (IM' i)) indices in
+         let new_states := zip_with (fun s t => fst (t Receive (s, Some m)))
+                                    states
+                                    transitions in
+         let eqs := equivocators new_states in
+         match otreshold with
+           | Some treshold =>
+             ((@sum_weights _ (Build_Measurable _ (fun idx => nth idx weights (exist _ 1%R _))) eqs) < treshold)%R
+           | None => True
+         end
+       end.
+  Next Obligation.
+    lra.
+  Defined.
+  
+  
+  Definition composite_elmo := @composite_vlsm Premessage index IndEqDec IM i0 composition_constraint.
+  Definition free_composite_elmo := @free_composite_vlsm Premessage index IndEqDec IM i0.
+
+  Lemma all_receive_observation_have_component_as_witness st m witness idx:
+    protocol_state_prop free_composite_elmo st ->
+    In (Cobservation Receive m witness) (observationsOf (st idx)) ->
+    witness = index_to_component idx.
+  Proof.
+    intros Hpsp Hin.
+    induction Hpsp using protocol_state_prop_ind.
+    - simpl in Hs. unfold composite_initial_state_prop in Hs.
+      assert (Hos: observationsOf (s idx) = []).
+      { apply Hs. }
+      rewrite Hos in Hin. simpl in Hin. inversion Hin.
+    - unfold protocol_transition in Ht.
+      destruct Ht as [Hvalid Ht].
+      unfold transition in Ht.
+      simpl in Ht.
+      destruct l as [i li].      
+      remember (vtransition (IM i) li (s i, om)) as VT.
+      destruct VT as [si'' om''].
+      unfold vtransition in HeqVT. simpl in HeqVT.
+
+      destruct (decide (i = idx)).
+      2: {
+        apply IHHpsp. clear IHHpsp.
+        inversion Ht. subst. clear Ht.
+        rewrite state_update_neq in Hin. apply nesym. exact n.
+        exact Hin.
+      }
+      subst i.
+      
+      destruct li, om; inversion HeqVT; subst; clear HeqVT;
+        inversion Ht; subst; clear Ht;
+        rewrite state_update_eq in Hin.
+      + apply in_app_or in Hin.
+        destruct Hin as [Hin|Hin]; [auto|].
+        simpl in Hin.
+        destruct Hin as [Hin|Hin]; inversion Hin; subst.
+        reflexivity.
+      + auto.
+      + auto.
+      + simpl in Hin.
+        apply in_app_or in Hin.
+        destruct Hin as [Hin|Hin]; [auto|].
+        simpl in Hin.
+        destruct Hin as [Hin|Hin]; inversion Hin.
+  Qed.
+
+  Instance free_composite_elmo_has_been_received_capability:
+    has_been_received_capability free_composite_elmo.
+  Proof.
+    unfold free_composite_elmo. unfold free_composite_vlsm.
+    eapply composite_has_been_received_capability.
+    { apply finite_index. }
+    intros i.
+    apply elmo_has_been_received_capability.
+  Defined.
+
+  Lemma has_receive_observation_implies_is_protocol st idx m:
+    protocol_state_prop free_composite_elmo st ->
+    In (Cobservation Receive m (index_to_component idx)) (observationsOf (st idx)) ->
+    protocol_message_prop free_composite_elmo m.
+  Proof.
+    intros Hpsp Hin.
+    pose proof (Hpsp' := pre_loaded_with_all_messages_protocol_state_prop _ _ Hpsp).
+    pose proof (Hhbr := @proper_received _ free_composite_elmo free_composite_elmo_has_been_received_capability _ Hpsp').
+    specialize (Hhbr m).
+    unfold has_been_received_prop in Hhbr.
+    unfold all_traces_have_message_prop in Hhbr.
+    apply proj1 in Hhbr.
+    unfold has_been_received in Hhbr.
+    unfold free_composite_elmo_has_been_received_capability in Hhbr.
+    simpl in Hhbr.
+    unfold composite_has_been_received in Hhbr.
+    assert (Htmp: exists i : index, @has_been_received _ (IM i) (elmo_has_been_received_capability addresses (index_to_component i) weights otreshold) (st i) m).
+    {
+      exists idx.
+      unfold has_been_received. unfold elmo_has_been_received_capability. simpl.
+      unfold elmo_has_been_received_oracle.
+      
+      apply (filter_in _ (isWitnessedBy (index_to_component idx))) in Hin.
+      2: { unfold isWitnessedBy. simpl.
+           destruct (bool_decide (index_to_component idx = index_to_component idx)) eqn:Heq.
+           reflexivity.
+           apply bool_decide_eq_false_1 in Heq. contradiction.
+      }
+      apply (filter_in _ isReceive) in Hin.
+      2: { reflexivity. }
+      
+      apply (@in_map _ _ messageOf _ _) in Hin.
+      exact Hin.
+    }
+    specialize (Hhbr Htmp). clear Htmp.
+    pose proof (Htmp := protocol_state_has_trace _ _ Hpsp).
+    destruct Htmp as [si [tr [Htrace Hlast]]].
+    specialize (Hhbr si tr).
+    
+    pose proof (Hp := (VLSM_incl_finite_protocol_trace _ _ (vlsm_incl_pre_loaded_with_all_messages_vlsm free_composite_elmo))). simpl in Hp.
+    unfold finite_protocol_trace in Hp.
+    pose proof (Htrace' := finite_protocol_trace_from_to_forget_last _ _ _ _ Htrace).
+    specialize (Hp _ _ (conj Htrace' Hlast)).
+    destruct Hp as [Hfrom Hsi].
+    unfold finite_protocol_trace_init_to in Hhbr.
+    specialize (Hhbr (conj (preloaded_weaken_finite_protocol_trace_from_to _ _ _ _ Htrace) Hlast)).
+    clear Hlast.
+    eapply protocol_trace_input_is_protocol.
+    apply Htrace'. unfold trace_has_message in Hhbr. exact Hhbr.
+  Qed.
+  
+  Lemma has_send_observation_implies_is_protocol st idx m author:
+    protocol_state_prop free_composite_elmo st ->
+    In (Cobservation Send m author) (observationsOf (st idx)) ->
+    protocol_message_prop free_composite_elmo m.
+  Proof.
+    intros Hpsp Hin.
+    induction Hpsp using protocol_state_prop_ind.
+    - simpl in Hs. unfold composite_initial_state_prop in Hs.
+      assert (Hos: observationsOf (s idx) = []).
+      { apply Hs. }
+      rewrite Hos in Hin.
+      simpl in Hin. inversion Hin.
+    - unfold protocol_transition in Ht.
+      destruct Ht as [Hvalid Ht].
+      unfold transition in Ht.
+      simpl in Ht.
+      destruct l as [i li].      
+      remember (vtransition (IM i) li (s i, om)) as VT.
+      destruct VT as [si'' om''].
+      unfold vtransition in HeqVT. simpl in HeqVT.
+
+      destruct (decide (i = idx)).
+      2: {
+        apply IHHpsp. clear IHHpsp.
+        inversion Ht. subst. clear Ht.
+        rewrite state_update_neq in Hin. apply nesym. exact n.
+        exact Hin.
+      }
+      subst i.
+
+      destruct li, om; inversion HeqVT; subst; clear HeqVT;
+        inversion Ht; subst; clear Ht;
+        rewrite state_update_eq in Hin.
+      + apply in_app_or in Hin.
+        simpl in Hin.
+        destruct Hin.
+        { apply IHHpsp. exact H. }
+        destruct H.
+        { inversion H. }
+        { inversion H. }
+      + apply IHHpsp. apply Hin.
+      + apply IHHpsp. apply Hin.
+      + simpl in Hin.
+        apply in_app_or in Hin.
+        destruct Hin.
+        { apply IHHpsp. exact H. }
+        simpl in H.
+        destruct H.
+        2: { inversion H. }
+        inversion H. subst. clear H.
+        unfold protocol_message_prop.
+        clear IHHpsp.
+        pose proof (Hgen := protocol_generated free_composite_elmo (existT _ idx Send)).
+        simpl in Hgen.
+        unfold protocol_valid in Hvalid.
+        destruct Hvalid as [Hpsp [_ Hvalid]].
+        destruct Hpsp as [m0 Hs].
+        specialize (Hgen s m0 Hs).
+        assert (Hinit: protocol_prop free_composite_elmo (fun=> Cprestate [], None)).
+        { apply protocol_initial. simpl. intros x. unfold vinitial_state_prop. simpl.
+          unfold elmo_initial_state_prop. reflexivity. simpl. exact I. }
+        specialize (Hgen _ _ Hinit). clear Hinit.
+        assert (Hvalid': constrained_composite_valid IM (free_constraint IM) (existT (fun=> Label) idx Send) (s, None)).
+        {
+          unfold constrained_composite_valid.
+          simpl.
+          unfold free_constraint.
+          split; [| exact I].
+          unfold vvalid. simpl. apply is_true_true.
+        }
+        specialize (Hgen Hvalid'). clear Hvalid'.
+        unfold vtransition in Hgen. simpl in Hgen.
+        eexists. apply Hgen.
+  Qed.
+  
+  Lemma protocol_state_satisfies_all_received_satisfy_isprotocol_prop st idx:
+    protocol_state_prop free_composite_elmo st ->
+    @all_received_satisfy_isprotocol_prop weights otreshold (observationsOf (st idx)).
+  Proof.
+    intros Hpsp.
+    induction Hpsp using protocol_state_prop_ind.
+    - simpl in Hs. unfold composite_initial_state_prop in Hs.
+      assert (Hos: observationsOf (s idx) = []).
+      { apply Hs. }
+      rewrite Hos.
+      unfold all_received_satisfy_isprotocol_prop.
+      apply Forall_nil.
+    - destruct l.
+      unfold protocol_transition in Ht.
+      destruct Ht as [Hvt Ht].
+      simpl in Ht.
+      remember (vtransition (IM x) v (s x, om)) as vt.
+      destruct vt as [si' o].
+      destruct (decide (x = idx)).
+      2: {
+        assert (Hsidx: s idx = s' idx).
+        {
+          inversion Ht. subst.
+          rewrite state_update_neq. apply nesym. exact n.
+          reflexivity.
+        }
+        rewrite Hsidx in IHHpsp.
+        exact IHHpsp.
+      }
+      subst x.
+      inversion Ht. subst. clear Ht.
+      rewrite state_update_eq.
+      unfold vtransition in Heqvt.
+      simpl in Heqvt.
+      destruct v,om; inversion Heqvt; clear Heqvt; subst.
+      4: { simpl.
+           unfold all_received_satisfy_isprotocol_prop.
+           apply Forall_app.
+           split; [exact IHHpsp|].
+           apply Forall_cons.
+           2: { apply Forall_nil. }
+           simpl.
+           exact is_true_true.
+      }
+      3: { exact IHHpsp. }
+      2: { exact IHHpsp. }
+      { simpl.
+        unfold all_received_satisfy_isprotocol_prop.
+        apply Forall_app.
+        split; [exact IHHpsp|].
+        apply Forall_cons.
+        2: { apply Forall_nil. }
+        simpl.
+        unfold protocol_valid in Hvt.
+        destruct Hvt as [[_ _] [_ Hvalid]].
+        unfold valid in Hvalid. simpl in Hvalid.
+        unfold constrained_composite_valid in Hvalid.
+        simpl in Hvalid. destruct Hvalid as [Hvalid _].
+        unfold vvalid in Hvalid. simpl in Hvalid.
+        apply andb_prop in Hvalid.
+        destruct Hvalid as [Hfn HisP].
+        exact HisP.
+      }
+  Qed.
+
+  Lemma protocol_state_contains_receive_implies_isProtocol st idx msg n0:
+    protocol_state_prop free_composite_elmo st ->
+    List.In (Cobservation Receive msg n0) (observationsOf (st idx)) ->
+    isProtocol (stateOf msg) (authorOf msg) weights otreshold.
+  Proof.
+    intros Hpsp Hin.
+    pose proof (H := protocol_state_satisfies_all_received_satisfy_isprotocol_prop st idx Hpsp).
+    unfold all_received_satisfy_isprotocol_prop in H.
+    eapply (proj1 (@Forall_forall Observation _ _)) in H.
+    2: apply Hin.
+    simpl in H. exact H.
+  Qed.
+
+  (* TODO s1 is reachable from s0 *)
+  Lemma protocol_message_was_sent_from_protocol_state s1 st author:
+    protocol_prop free_composite_elmo (s1, Some (Cpremessage st author)) ->
+    (
+    exists s0,
+      protocol_state_prop free_composite_elmo s0
+      /\ (s0 (component_to_index author)) = st
+    ) /\ (List.In (Cobservation Send (Cpremessage st author) author) (observationsOf (s1 (component_to_index author))))
+  .
+  Proof.
+    intros H.
+    inversion H; subst; clear H.
+    { simpl in Hom. unfold composite_initial_message_prop in Hom.
+      destruct Hom as [n [mi Hmi]].
+      unfold vinitial_message in mi. unfold initial_message in mi.
+      simpl in mi.
+      pose proof (proj2_sig mi) as H0. simpl in H0. inversion H0.
+    }
+    destruct l as [i li].
+    remember (vtransition (IM i) li (s i, om)) as VT.
+    destruct VT as [st' om']. inversion H1. subst. clear H1.
+    unfold vtransition in HeqVT. simpl in HeqVT.
+    destruct li,om; inversion HeqVT; subst; clear HeqVT.
+    rewrite index_to_component_to_index.
+    split.
+    - unfold protocol_state_prop.
+      eexists. split. eexists. apply Hps. reflexivity.
+    - rewrite state_update_eq. simpl.
+      apply in_or_app. right. simpl. left. reflexivity.
+  Qed.
+
+  Lemma isProtocol_last_fullNode l p n1 n0 component:
+    n1 <> component ->
+    isProtocol (Cprestate (l ++ [Cobservation Receive (Cpremessage p n1) n0]))
+               component weights otreshold ->
+    fullNode (Cpremessage p n1) l component.
+  Proof.
+    intros Hneq Hproto.
+    unfold isProtocol in Hproto. simpl in Hproto.
+    
+    rewrite fold_left_app in Hproto. simpl in Hproto.
+    remember (fold_left
+                (isProtocol_step component weights otreshold                 
+                                 (l ++ [Cobservation Receive (Cpremessage p n1) n0])) l   
+                (true, 0, map (fun=> Cprestate []) weights, [])) as FL.
+    unfold isProtocol_step in Hproto at 1.
+    destruct FL as [[[b i] curState] curEq].
+    destruct b; simpl in Hproto.
+    2: { inversion Hproto. }
+    destruct (bool_decide (n0 = component)); simpl in Hproto.
+    2: { inversion Hproto. }
+    destruct (bool_decide (n1 = component)) eqn:Heq; simpl in Hproto.
+    { apply bool_decide_eq_true in Heq. contradiction. }
+    
+    pose proof (Htmp := isProtocol_step_fold_result_true_idx component weights otreshold).
+    specialize (Htmp (l ++ [Cobservation Receive (Cpremessage p n1) n0])).
+    specialize (Htmp l (true, 0, map (fun=> Cprestate []) weights, [])).
+    simpl in Htmp.
+    rewrite -HeqFL in Htmp. specialize (Htmp (eq_refl _)). subst i.
+    rewrite firstn_app in Hproto. rewrite Nat.sub_diag in Hproto. simpl in Hproto.
+    rewrite app_nil_r in Hproto. rewrite firstn_all in Hproto.
+
+    remember (fullNode (Cpremessage p n1) l component) as FN.
+    destruct FN; simpl in Hproto.
+    2: { inversion Hproto. }
+    exact is_true_true.
+  Qed.
+
+
+  Lemma isProtocol_last_sendInPrefix l p n0 component:
+    isProtocol (Cprestate (l ++ [Cobservation Receive (Cpremessage p component) n0]))
+               component weights otreshold ->
+    List.In (Cobservation Send (Cpremessage p component) component) l.
+  Proof.
+    intros Hproto.
+    unfold isProtocol in Hproto. simpl in Hproto.
+    
+    rewrite fold_left_app in Hproto. simpl in Hproto.
+    remember (fold_left
+                (isProtocol_step component weights otreshold                 
+                                 (l ++ [Cobservation Receive (Cpremessage p component) n0])) l   
+                (true, 0, map (fun=> Cprestate []) weights, [])) as FL.
+    unfold isProtocol_step in Hproto at 1.
+    destruct FL as [[[b i] curState] curEq].
+    destruct b; simpl in Hproto.
+    2: { inversion Hproto. }
+    destruct (bool_decide (n0 = component)); simpl in Hproto.
+    2: { inversion Hproto. }
+    destruct (bool_decide (component = component)) eqn:Heq; simpl in Hproto.
+    2: { apply bool_decide_eq_false in Heq. contradiction. }
+    apply bool_decide_eq_true in Hproto.
+
+    pose proof (Htmp := isProtocol_step_fold_result_true_idx component weights otreshold).
+    specialize (Htmp (l ++ [Cobservation Receive (Cpremessage p component) n0])).
+    specialize (Htmp l (true, 0, map (fun=> Cprestate []) weights, [])).
+    simpl in Htmp.
+    rewrite -HeqFL in Htmp. specialize (Htmp (eq_refl _)). subst i.
+    rewrite firstn_app in Hproto. rewrite Nat.sub_diag in Hproto. simpl in Hproto.
+    rewrite app_nil_r in Hproto. rewrite firstn_all in Hproto.
+    exact Hproto.
+  Qed.
+
+  Lemma sent_is_protocol st m component:
+    address_valid component ->
+    protocol_state_prop free_composite_elmo st ->
+    In (Cobservation Send m component) (observationsOf (st (component_to_index component))) ->
+    protocol_message_prop free_composite_elmo m.
+  Proof.
+    intros Haddr Hpsp Hin.
+    induction Hpsp using protocol_state_prop_ind.
+    - simpl in Hs. unfold composite_initial_state_prop in Hs.
+      assert (Hos: observationsOf (s (component_to_index component)) = []).
+      { apply Hs. }
+      rewrite Hos in Hin. simpl in Hin. inversion Hin.
+    - unfold protocol_transition in Ht.
+      destruct Ht as [Hvalid Ht].
+      unfold transition in Ht. simpl in Ht.
+      destruct l as [i li].
+      remember (vtransition (IM i) li (s i, om)) as VT.
+      destruct VT as [si'' om'']. inversion Ht. subst. clear Ht.
+      
+      destruct (decide (component_to_index component = i)).
+      2: { rewrite state_update_neq in Hin.
+           { exact n. }
+           apply IHHpsp. apply Hin.
+      }
+      subst i.
+      rewrite state_update_eq in Hin.
+      unfold protocol_valid in Hvalid. destruct Hvalid as [Hpsp [Hopmp Hvalid]].
+      unfold vtransition in HeqVT. simpl in HeqVT.
+      destruct li,om; inversion HeqVT; subst; clear HeqVT.
+      + simpl in Hin. apply in_app_or in Hin.
+        simpl in Hin. destruct Hin as [Hin|[Hin|Hin]].
+        3: { inversion Hin. }
+        2: { rewrite component_to_index_to_component in Hin. exact Haddr. inversion Hin. }
+        auto.
+      + auto.
+      + auto.
+      + simpl in Hin.
+        rewrite component_to_index_to_component in Hin.
+        { exact Haddr. }
+        apply in_app_or in Hin.
+        simpl in Hin.
+        destruct Hin as [Hin|[Hin|Hin]].
+        3: { inversion Hin. }
+        2: { inversion Hin. subst. clear Hin.
+             clear IHHpsp.
+             Check protocol_generated.
+             pose proof (Hgen := protocol_generated free_composite_elmo (existT _ (component_to_index component) Send)).
+             destruct Hpsp as [_om Hpsp].
+             specialize (Hgen _ _om Hpsp).
+             assert (Hpi: protocol_prop free_composite_elmo (fun=> Cprestate [], None)).
+             { apply protocol_initial. simpl. intros x. reflexivity. reflexivity. }
+             specialize (Hgen _ _ Hpi Hvalid).
+             clear Hpi.
+             unfold transition in Hgen. simpl in Hgen.
+             rewrite component_to_index_to_component in Hgen.
+             { exact Haddr. }
+             eexists. apply Hgen.
+        }
+        auto.
+  Qed.
+
+  
+  Lemma fullNode_appObservation m component l ob:
+    fullNode m l component = true ->
+    fullNode m (l ++ [ob]) component = true.
+  Proof.
+    intros H.
+
+    unfold fullNode in H. apply Forall_fold_right_bool in H.
+    unfold fullNode. apply Forall_fold_right_bool.
+    induction H.
+    - apply Forall_nil.
+    - apply Forall_cons.
+      2: { auto. }
+      clear H0 IHForall.
+      destruct (decide (authorOf (messageOf x) = component)); simpl in H; simpl.
+      * apply bool_decide_eq_true_1 in H. apply bool_decide_eq_true_2.
+        apply in_or_app. left. exact H.
+      * apply bool_decide_eq_true_1 in H. apply bool_decide_eq_true_2.
+        apply in_or_app. left. exact H.
+  Qed.
+
+  (* All observations in a state have the same witness - which is the address of the node. *)
+  Lemma observationsHaveSameWitness st component ob:
+    address_valid component ->
+    protocol_state_prop free_composite_elmo st ->
+    In ob (observationsOf (st (component_to_index component))) ->
+    witnessOf ob = component.
+  Proof.
+    intros Haddr Hpsp Hin.
+    induction Hpsp using protocol_state_prop_ind.
+    - simpl in Hs. unfold composite_initial_state_prop in Hs.
+      assert (Hos: observationsOf (s (component_to_index component)) = []).
+      { apply Hs. }
+      rewrite Hos in Hin. simpl in Hin. inversion Hin.
+    - unfold protocol_transition in Ht.
+      destruct Ht as [Hvalid Ht].
+      unfold transition in Ht. simpl in Ht.
+      destruct l as [i li].
+      remember (vtransition (IM i) li (s i, om)) as VT.
+      destruct VT as [si'' om'']. inversion Ht. subst om'' s'. clear Ht.
+      
+      destruct (decide (component_to_index component = i)).
+      2: { rewrite state_update_neq in Hin.
+           { exact n. }
+           auto.
+      }
+      subst i.
+      rewrite state_update_eq in Hin.
+
+      unfold vtransition in HeqVT.
+      simpl in HeqVT.
+      destruct li,om; inversion HeqVT; clear HeqVT; subst; auto.
+      + simpl in Hin. apply in_app_or in Hin.
+        destruct Hin as [Hin|Hin];[auto|].
+        simpl in Hin.
+        destruct Hin as [Hin|Hin];[|inversion Hin].
+        subst ob. simpl.
+        rewrite component_to_index_to_component.
+        { exact Haddr. }
+        reflexivity.
+      + simpl in Hin.
+        apply in_app_or in Hin.
+        destruct Hin as [Hin|Hin];[auto|].
+        simpl in Hin.
+        destruct Hin as [Hin|Hin];[|inversion Hin].
+        subst ob. simpl.
+        rewrite component_to_index_to_component.
+        { exact Haddr. }
+        reflexivity.
+  Qed.
+  
+  (* All observations with sender other than the component are Receive observations.  *)
+  Lemma observationsWithAddressNotComponentAreReceive st component ob:
+    address_valid component ->
+    protocol_state_prop free_composite_elmo st ->
+    In ob (observationsOf (st (component_to_index component))) ->
+    authorOf (messageOf ob) <> component ->
+    labelOf ob = Receive.
+  Proof.
+    intros Haddr Hpsp Hin Hauthor.
+    induction Hpsp using protocol_state_prop_ind.
+    - simpl in Hs. unfold composite_initial_state_prop in Hs.
+      assert (Hos: observationsOf (s (component_to_index component)) = []).
+      { apply Hs. }
+      rewrite Hos in Hin. simpl in Hin. inversion Hin.
+    - unfold protocol_transition in Ht.
+      destruct Ht as [Hvalid Ht].
+      unfold transition in Ht. simpl in Ht.
+      destruct l as [i li].
+      remember (vtransition (IM i) li (s i, om)) as VT.
+      destruct VT as [si'' om'']. inversion Ht. subst om'' s'. clear Ht.
+      
+      destruct (decide (component_to_index component = i)).
+      2: { rewrite state_update_neq in Hin.
+           { exact n. }
+           auto.
+      }
+      subst i.
+      rewrite state_update_eq in Hin.
+
+      unfold vtransition in HeqVT.
+      simpl in HeqVT.
+      destruct li,om; inversion HeqVT; clear HeqVT; subst; auto.
+      + simpl in Hin. apply in_app_or in Hin.
+        destruct Hin as [Hin|Hin];[auto|]. clear IHHpsp.
+        simpl in Hin.
+        destruct Hin as [Hin|Hin];[|inversion Hin].
+        subst ob. reflexivity.
+      + simpl in Hin.
+        apply in_app_or in Hin.
+        destruct Hin as [Hin|Hin];[auto|]. clear IHHpsp.
+        simpl in Hin.
+        destruct Hin as [Hin|Hin];[|inversion Hin].
+        subst ob. simpl.
+        simpl in Hauthor.
+        rewrite component_to_index_to_component in Hauthor.
+        { exact Haddr. }
+        contradiction.
+  Qed.
+
+  Lemma trace_from_to_impl_observations_prefix s1 s2 (tr : list transition_item) component:
+    let i := component_to_index component in
+    finite_protocol_trace_from_to (pre_loaded_with_all_messages_vlsm (IM i)) s1 s2 tr ->
+    exists (n : nat),
+      length (observationsOf s2) >= n /\
+      list_prefix (observationsOf s2) n = observationsOf s1.
+  Proof.
+    intros i.
+    intros Htr.
+    move: s1 s2 component i Htr.
+    induction tr; intros s1 s2 component i Htr.
+    - inversion Htr. subst.
+      exists (length (observationsOf s2)).
+      split. lia.
+      rewrite -> list_prefix_all by lia.
+      reflexivity.
+    - inversion Htr. subst. clear Htr.
+      rename l into lbl.
+      (*destruct l as [idx lbl].*)
+      unfold protocol_transition in H4.
+      simpl in H4.
+      destruct H4 as [[[opmp Hopmp] [Hiom Hvalid]] Htrans].
+      rename H3 into Hss2.
+      remember (vtransition (IM i) lbl (s1, iom)) as VT.
+      destruct VT as [s1' oom'].
+      inversion Htrans. subst. clear Htrans.
+      unfold vtransition in HeqVT. simpl in HeqVT.
+      destruct lbl,iom; inversion HeqVT; subst; clear HeqVT
+      + simpl.
+        pose proof (IH := IHtr _ _ component i Hss2).
+        destruct IH as [n Hn].
+
+        (* n <> 0 *)
+        destruct n.
+        { rewrite list_prefix_0 in Hn. simpl in Hn.
+          destruct Hn as [_ Hn].
+          apply eq_sym in Hn.
+          destruct (last_not_null _ _ Hn).
+        }
+        simpl in Hn.
+        destruct Hn as [Hl Hn].
+        
+        apply list_prefix_S in Hn.
+        2: { exact Hl. }
+        exists n. split. lia. apply Hn.
+      + eauto.
+      + eauto.
+      + pose proof (IH := IHtr _ _ component i Hss2).
+        destruct IH as [n Hn].
+        (* n <> 0 *)
+        destruct n.
+        { rewrite list_prefix_0 in Hn. simpl in Hn.
+          destruct Hn as [_ Hn].
+          apply eq_sym in Hn.
+          destruct (last_not_null _ _ Hn).
+        }
+        simpl in Hn.
+        destruct Hn as [Hl Hn].
+        
+        apply list_prefix_S in Hn.
+        2: { exact Hl. }
+        exists n. split. lia. apply Hn. 
+  Qed.
+  
+
+  (* If there is a [Cobservation Receive m component], then there is also
+                   [Cobservation Send m component]. *)
+  Lemma received_from_self_implies_sent st s component:
+    address_valid component ->
+    protocol_state_prop free_composite_elmo st ->
+    let obs := observationsOf (st (component_to_index component)) in
+    In (Cobservation Receive (Cpremessage s component) component) obs ->
+    In (Cobservation Send (Cpremessage s component) component) obs.
+  Proof.
+    simpl.
+    intros Haddr Hpsp Hrecv.
+    assert (Hhbr:
+              @has_been_received
+                _
+                (IM (component_to_index component))
+                (elmo_has_been_received_capability _ _ _ _)
+                (st (component_to_index component))
+                (Cpremessage s component)
+           ).
+    {
+      simpl.
+      unfold elmo_has_been_received_oracle.
+      rewrite component_to_index_to_component.
+      { exact Haddr. }
+      apply (filter_in _ (isWitnessedBy component)) in Hrecv.
+      2: { unfold isWitnessedBy. simpl.
+           destruct (bool_decide (component = component)) eqn:Heq.
+           reflexivity.
+           apply bool_decide_eq_false_1 in Heq. contradiction.
+      }
+      
+      apply (filter_in _ isReceive) in Hrecv.
+      2: { reflexivity. }
+      Check in_map.
+      apply (in_map messageOf) in Hrecv.
+      exact Hrecv.
+    }
+    (* Maybe if we had the check that the message was already sent... *)
+    (*clear Hrecv.*)
+
+    remember (component_to_index component) as i.
+    assert (Hpspi: protocol_state_prop (pre_loaded_with_all_messages_vlsm (IM i)) (st i)).
+    { apply preloaded_composed_protocol_state.
+      apply pre_loaded_with_all_messages_protocol_state_prop.
+      exact Hpsp.
+    }
+
+
+    pose proof (Htmp := has_been_received_in_state_preloaded _ _ _ _ Hpspi Hhbr).
+    (*pose proof (Htmp := has_been_received_in_state _ _ _ _ Hpsp Hhbr).*)
+    destruct Htmp as [s0 [item [tr [Hin Hfpt]]]].
+    (* We will need Hfpt' later for monotonicity. *)
+    pose proof (Hfpt' := Hfpt).
+    inversion Hfpt. subst tl f s' item. clear Hfpt.
+    simpl in Hin. subst iom.
+    (* We will use H3 later for monotonicity. *)
+    
+    rename H4 into Hpt.
+    unfold protocol_transition in Hpt.
+    destruct Hpt as [Hvalid Hs1].
+    simpl in Hvalid.
+    destruct Hvalid as [Hs0 [Hmsg Hvalid]].
+    unfold constrained_composite_valid in Hvalid.
+    (*destruct Hvalid as [Hvalid _]*)
+    simpl in Hvalid.
+    (*destruct l as [i li].*)
+    unfold vvalid in Hvalid. simpl in Hvalid.
+    destruct l; [| inversion Hvalid].
+
+    apply andb_prop in Hvalid. destruct Hvalid as [Hvalid _].
+    apply andb_prop in Hvalid. destruct Hvalid as [_ Hvalid].
+    rewrite Heqi in Hvalid.
+    rewrite component_to_index_to_component in Hvalid.
+    { exact Haddr. }
+    destruct (decide (component = component)).
+    2: { contradiction. }
+    simpl in Hvalid. clear e.
+    apply bool_decide_eq_true_1 in Hvalid.
+    subst i.
+    pose proof (Hprefix := trace_from_to_impl_observations_prefix _ _ _ _ Hfpt').
+    destruct Hprefix as [n [_ Hprefix]].
+    rewrite -Hprefix in Hvalid.
+    eapply In_list_prefix.
+    apply Hvalid.
+  Qed.
+
+
+  Lemma protocol_message_has_valid_sender p address:
+    protocol_message_prop free_composite_elmo (Cpremessage p address) ->
+    address_valid address.
+  Proof.
+    intros Hpmp.
+    apply protocol_message_prop_iff in Hpmp.
+    destruct Hpmp.
+    - destruct H as [im Him].
+      unfold initial_message in im.
+      pose proof (proj2_sig im). simpl in H. unfold composite_initial_message_prop in H.
+      destruct H as [n [mi Hmi]].
+      unfold vinitial_message,initial_message in mi.
+      pose proof (proj2_sig mi). simpl in H. inversion H.
+    - destruct H as [l [som [s' Htrans]]].
+      destruct l.
+      unfold protocol_transition in Htrans.
+      destruct Htrans as [_ Htrans].
+      unfold transition in Htrans.
+      simpl in Htrans.
+      unfold composite_transition in Htrans. destruct som.
+      remember (vtransition (IM x) v (s x, o)) as VT.
+      destruct VT. inversion Htrans. subst. clear Htrans.
+      unfold vtransition,transition in HeqVT.
+      simpl in HeqVT.
+      destruct v,o; inversion HeqVT. clear HeqVT. subst.
+      unfold address_valid.
+      unfold index_to_component.
+      apply findInList_found.
+      apply finite_index.
+  Qed.
+  
+  
+  Lemma sent_is_fullNode st m component component':
+    address_valid component ->
+    protocol_state_prop free_composite_elmo st ->
+    authorOf m = component ->
+    let st' := st (component_to_index component) in
+    In (Cobservation Send m component') (observationsOf st') ->
+    fullNode m (observationsOf st') component = true.
+  Proof.
+    intros Haddr Hpsp Hauthor st' Hin.
+    induction Hpsp using protocol_state_prop_ind.
+    - simpl in Hs. unfold composite_initial_state_prop in Hs.
+      assert (Hos: observationsOf (s (component_to_index component)) = []).
+      { apply Hs. }
+      rewrite Hos in Hin. simpl in Hin. inversion Hin.
+    - unfold protocol_transition in Ht.
+      destruct Ht as [Hvalid Ht].
+      unfold transition in Ht. simpl in Ht.
+      destruct l as [i li].
+      remember (vtransition (IM i) li (s i, om)) as VT.
+      destruct VT as [si'' om'']. inversion Ht. subst om'' s'. clear Ht.
+      
+      destruct (decide (component_to_index component = i)).
+      2: { unfold st' in Hin.
+           rewrite state_update_neq in Hin.
+           { exact n. }
+           unfold st'.
+           rewrite state_update_neq.
+           { exact n. }
+           simpl in IHHpsp.
+           (*unfold ob. unfold st'
+           rewrite state_update_neq.
+           { exact n. }*)
+           apply IHHpsp.
+           apply Hin.
+      }
+      subst i.
+      unfold st' in Hin.
+      rewrite state_update_eq in Hin.
+      unfold protocol_valid in Hvalid. destruct Hvalid as [Hpsp [Hopmp Hvalid]].
+      unfold vtransition in HeqVT. simpl in HeqVT.
+      destruct li,om; inversion HeqVT; subst; clear HeqVT.
+      + simpl in Hin. apply in_app_or in Hin.
+        simpl in Hin. destruct Hin as [Hin|[Hin|Hin]].
+        3: { inversion Hin. }
+        2: { rewrite component_to_index_to_component in Hin. exact Haddr. inversion Hin. }
+        unfold st'.
+        rewrite component_to_index_to_component.
+        { exact Haddr. }
+        rewrite state_update_eq.
+        specialize (IHHpsp Hin). clear Hin. simpl. simpl in IHHpsp.
+        unfold st' in *. clear st'.
+        (*unfold ob in *. clear ob.
+        rewrite component_to_index_to_component.
+        { exact Haddr. }
+        rewrite state_update_eq.*)
+        apply fullNode_appObservation. exact IHHpsp.
+      + unfold st'. rewrite state_update_eq. auto.
+      + unfold st'. rewrite state_update_eq. auto.
+      + unfold st'. rewrite state_update_eq.
+        simpl in Hin.
+        rewrite component_to_index_to_component in Hin.
+        { exact Haddr. }
+        rewrite component_to_index_to_component.
+        { exact Haddr. }
+        apply in_app_or in Hin.
+        simpl in Hin.
+        destruct Hin as [Hin|[Hin|Hin]]; simpl.
+        3: { inversion Hin. }
+        2: { simpl. inversion Hin. clear Hin.
+             simpl.
+             destruct m. simpl. simpl in H0.
+             inversion H0. clear H0. subst p.
+             simpl in IHHpsp.
+             apply fullNode_appObservation.
+             unfold fullNode.
+             simpl.
+             apply Forall_fold_right_bool.
+             remember (observationsOf (s (component_to_index n))) as obs.
+             apply Forall_forall.
+             intros x Hx. destruct x. simpl. destruct p. simpl.
+
+             (* Some facts:
+                1. All observations in a state have the same witness - which is the address
+                  of the node (lemma [observationsHaveSameWitness]).
+                2. If there is a [Cobservation Receive m component], then there is also
+                   [Cobservation Send m component].
+                3. All observations with sender other than the component are Receive observations.
+                Then the following cases might happen:
+                * n1 = n -> Either l=Send, and we can use Hx. Or l=Receive, and by (2), there is some Send in obs.
+                * n1 <> n -> the message was sent by some other node, and by (3) we have l=Receive, and we can use Hx.
+                *)
+             simpl in Haddr.
+             
+             assert (n0 = n).
+             { rewrite Heqobs in Hx.
+               pose proof (observationsHaveSameWitness s n _ Haddr Hpsp Hx).
+               simpl in H. exact H.
+             }
+             subst n0.
+
+             simpl in Hvalid. clear Hvalid. (* a Send transition is trivially valid *)
+             destruct (decide (n1 = n)); simpl; apply bool_decide_eq_true_2.
+             - subst n1.
+               destruct l.
+               + rewrite Heqobs.
+                 apply received_from_self_implies_sent.
+                 { exact Haddr. }
+                 { exact Hpsp. }
+                 rewrite Heqobs in Hx.
+                 exact Hx.
+               + exact Hx.
+             - assert (l = Receive).
+               {
+                 pose proof (H := observationsWithAddressNotComponentAreReceive).
+                 rewrite Heqobs in Hx.
+                 specialize (H _ _ _ Haddr Hpsp Hx).
+                 simpl in H.
+                 auto.
+               }
+               subst l. exact Hx.
+               
+        }
+        apply fullNode_appObservation. auto.
+  Qed.
+
+
+  (* FIXME: Duplicate of isProtocol_last_sendInPrefix *)
+  Lemma isProtocol_last_receive_impl_send l p n n0:
+    isProtocol (Cprestate (l ++ [Cobservation Receive (Cpremessage p n) n0]))
+               n weights otreshold ->
+    In (Cobservation Send (Cpremessage p n) n) l.
+  Proof.
+    intros H.
+    unfold isProtocol in H.
+    rewrite fold_left_app in H. simpl in H.
+    remember (fold_left
+          (isProtocol_step n weights otreshold (l ++ [Cobservation Receive (Cpremessage p n) n0])) l
+          (true, 0, map (fun=> Cprestate []) weights, [])) as FL.
+    inversion H.
+    pose proof (isProtocol_step_result_true _ _ _ _ _ _ H1).
+    destruct FL as [[[b n'] ps] sn]. simpl in H0. subst b.
+    clear -H1. unfold isProtocol_step in H1. simpl in H1.
+    destruct (bool_decide (n0 = n)); simpl in H1.
+    2: { inversion H1. }
+    destruct (bool_decide (n = n)) eqn:Heq.
+    2: { apply bool_decide_eq_false in Heq. contradiction. }
+    clear Heq.
+    simpl in H1. apply bool_decide_eq_true in H1.
+    rewrite firstn_app in H1.
+    apply in_app_or in H1.
+    destruct H1.
+    2: { Search In firstn. apply In_firstn in H. simpl in H.
+         destruct H; [|contradiction]. inversion H.
+    }
+    eapply In_firstn. apply H.
+  Qed.
+
+  Lemma protocol_strip_last l x n:
+    protocol_message_prop free_composite_elmo (Cpremessage (Cprestate (l ++ [x])) n) ->
+    protocol_message_prop free_composite_elmo (Cpremessage (Cprestate l) n).
+  Proof.
+    intros H.
+    Check exists_first. (* <-- TODO remove *)
+    Check Exists_first.
+    Check existsb_first.
+
+    (* TODO write Exists_last *)
+    
+    Search "exist" "++"
+    (* [Cpremessage (Cprestate (l ++ [x]))] must have been sent from some protocol state
+    [s] such that [s n = Cprestate (l ++ [x])].
+        Now if there were no transition to [s n] from some protocol state [s'] satisfying
+        [s' n = Cprestate l], then the [n]th projection of any state on any trace leading to [s]
+        would be [Cprestate (l ++ [x])] - even the initial state. But initial state is empty!
+        That is a contradiction, and therefore there must be some such [s'].
+
+        Consider a trace [is, tr] leading to [s]. There must be some position [i] such that
+        [map label (nth_error tr i) = Some (n, Receive)]
+        and [finite_trace_nth is tr i = Some l].
+        Well, it depends who's observation is [x].
+        At the very least, there must be some position [i] such that
+        and [finite_trace_nth is tr i = Some l] - because the state can only grow
+        and starts in empty state.
+
+        We can then extend the i-prefix of tr with label [(n, Send)] and get
+        the protocol message (Cpremessage (Cprestate l) n).
+
+     *)
+
+    destruct H as [s Hproto].
+    pose proof (Htrace := protocol_is_trace free_composite_elmo _ _ Hproto).
+    destruct Htrace.
+        (* TODO prove a lemma saying that all messages from the initial state contain only the empty state.
+       From that it should follow that s is not initial.
+       For that it could be helpful to prove that (1) initial state is empty, and (2) composite initial state is a collection of empty states.
+*)
+    
+    Check nth_error.
+    Print transition_item.
+    Search state list transition_item.
+    Check trace_is_protocol_prop.
+
+    
+    apply protocol_message_prop_iff in H.
+    destruct H.
+    { destruct H as [im H].
+      (* TODO extract this proof out. *)
+      unfold initial_message in im.
+      pose proof (proj2_sig im). rewrite -H in H0. simpl in H0.
+      unfold composite_initial_message_prop in H0. destruct H0 as [n0 [mi Hmi]].
+      unfold vinitial_message,initial_message in mi.
+      pose proof (proj2_sig mi). rewrite Hmi in H0. simpl in H0. inversion H0.
+    }
+    destruct H as [s Hproto].
+    induction Hproto usin
+  Abort.
+
+  Lemma protocol_implies_isProtocol m:
+    protocol_message_prop free_composite_elmo m ->
+    isProtocol (stateOf m) (authorOf m) weights otreshold.
+  Proof.
+    intros H.
+    destruct m. destruct p.
+    induction l using rev_ind; simpl.
+    - unfold isProtocol. simpl. reflexivity.
+    - 
+  Abort.
+  
+  
+  Lemma isProtocol_implies_protocol component st m:
+    otreshold = None ->
+    address_valid component ->
+    protocol_state_prop free_composite_elmo st ->
+    fullNode m (observationsOf (st (component_to_index component))) component ->
+    address_valid (authorOf m) ->
+    isProtocol (stateOf m) (authorOf m) weights otreshold  ->
+    protocol_message_prop free_composite_elmo m.
+  Proof.
+    intros HnoEquivCheck Hcomval Hpsp Hfull Haddr Hproto.
+    destruct m. destruct p. simpl.
+    pose proof (Hob := isProtocol_implies_ob_sent_contains_previous_prop _ _ _ _ Hproto).
+
+    move: n Haddr Hproto Hfull.
+    induction l using rev_ind; intros n Haddr Hproto Hfull.
+    - simpl in Hproto.
+      unfold protocol_message_prop.
+      simpl.
+      
+      (*set (mk_vlsm (elmo_vlsm_machine n weights treshold)) as vlsm.*)
+      pose proof (Hgen := protocol_generated free_composite_elmo).
+      simpl in Hgen.
+      Check (existT _ n Send).
+      (* We need to turn `n` into index *)
+      unfold _composite_label in Hgen.
+      specialize (Hgen (existT _ (component_to_index n) Send)).
+      eexists.
+      simpl in Hgen.
+      assert (Hpp0: protocol_prop free_composite_elmo (fun=> Cprestate [], None)).
+      { apply protocol_initial.
+        simpl. unfold composite_initial_state_prop.
+        intros n0. reflexivity.
+        reflexivity.
+      }
+      specialize (Hgen _ _ Hpp0). clear Hpp0.
+
+      specialize (Hgen (fun=> Cprestate []) None).
+      simpl in Hgen.
+      simpl in Haddr.
+      rewrite component_to_index_to_component in Hgen.
+      { exact Haddr. }
+      apply Hgen.
+      2: { unfold constrained_composite_valid.
+           split.
+           2: { unfold free_constraint. exact I. }
+           unfold composite_valid.
+           unfold vvalid. simpl. auto.
+      }
+      clear Hgen.
+      apply protocol_initial.
+      2: { reflexivity. }
+      intros x. unfold vinitial_state_prop. simpl. reflexivity.
+    - (* Step *)
+      pose proof (Hproto' := Hproto).
+      destruct x.
+      unfold isProtocol in Hproto. simpl in Hproto.
+      rewrite fold_left_app in Hproto. simpl in Hproto.
+      unfold isProtocol_step in Hproto at 1.
+      remember (fold_left (isProtocol_step n weights otreshold (l ++ [Cobservation l0 p n0])) l
+                          (true, 0, map (fun=> Cprestate []) weights, []))
+        as fl.
+      destruct fl as [[[b n'] pss] sn].
+      simpl in Hproto.
+      destruct b.
+      2: { simpl in Hproto. inversion Hproto. }
+      destruct (bool_decide (n0 = n)).
+      2: { simpl in Hproto. inversion Hproto. }
+      simpl in Hproto.
+      destruct p. simpl in Hproto.
+      destruct (bool_decide (n1 = n)), l0.
+      + simpl in Hproto.
+        admit.
+      + simpl in *.
+        admit.
+      + destruct (fullNode (Cpremessage p n1) (firstn n' (l ++ [Cobservation Receive (Cpremessage p n1) n0])) n).
+        2: { simpl in Hproto. inversion Hproto. }
+        simpl in Hproto. simpl in Heqfl.
+        remember (isProtocol_step n weights otreshold) as step.
+        (* We want to use Heqfl as the premise of IHl. But to do that, we must get rid
+         of the "++ [...]" part. *)
+        
+        (*
+      simpl in Hproto.
+      destruct (update (Cpremessage p n1) n weights treshold pss sn).
+      destruct p0. simpl in Hproto. Search b.
+         *)
+        (* Not useful. Clear it. *)
+        clear Hproto.
+        set (fold_left (step (l ++ [Cobservation Receive (Cpremessage p n1) n0])) l
+                       (true, 0, map (fun=> Cprestate []) weights, [])) as FL.
+        assert (HFLtrue: FL.1.1.1 = true).
+        { unfold FL. rewrite -Heqfl. reflexivity. }
+
+        subst step.
+        (*unfold FL in HFLtrue.*)
+        pose proof (Htmp := fold_isProtocol_step_app _ _ _ _ _ _ _ _ Hob HFLtrue).
+        unfold FL in HFLtrue.
+        rewrite Htmp in HFLtrue.
+        apply ob_sent_contains_previous_prop_app in Hob.
+        destruct Hob as [Hob _].
+        specialize (IHl Hob).
+        simpl in IHl.
+        simpl in Haddr.
+        
+        pose proof (IHl' := IHl n Haddr HFLtrue).
+        clear FL Heqfl Htmp HFLtrue.
+        clear n' pss sn.
+        simpl in IHl'.
+        simpl in Hproto'.
+        (*specialize (IHl (isProtocol_last _ _ _ _ _ Hproto') Hob).*)
+        clear Hob.
+        specialize (IHl' (fullNode_appone _ _ _ _ _ Hfull)).
+        (****)
+        destruct IHl' as [s Hs].
+        unfold protocol_message_prop.
+        (* Since [Cpremessage (Cprestate l) n] is not an initial message,
+         the message must be an output of the transition function, together with the state [s].
+         *)
+        inversion Hs; subst.
+        { simpl in Hom. destruct Hom as [i [mi Hmi]].
+          unfold vinitial_message in mi.
+          unfold initial_message in mi.
+          pose proof (Hsv := svalP mi).
+          rewrite Hmi in Hsv.
+          simpl in Hsv.
+          inversion Hsv.
+        }
+        destruct l0.
+        rename x into idx.
+        rename v into lbl.
+        remember (observationsOf (st (component_to_index component))) as obs.
+
+        (* I want to prove the goal using [protocol_generated].
+           I.e., there needs to be a state [Sx] from which a transition goes to some state [s1]
+           and  generates the message
+           [Cpremessage (Cprestate (l ++ [Cobservation Receive (Cpremessage p n1) n0]))].
+           That means that the composite state Sx must satisfy
+           [Sx n0 = (Cprestate (l ++ [Cobservation Receive (Cpremessage p n1) n0]))].
+           But in order to get into this state, there must be a protocol state [Sy]
+           that is the same at all components as Sx, except at the component n0, where
+           [Sy n0 = (Cprestate l)]; there must be the protocol message
+           [Cpremessage p n1] floating around.
+
+           How do we prove that [Cpremessage p n1] is a protocol message?
+           Either [n1 <> component], and then by Hfull,
+             [In (Cobservation Receive (Cpremessage p n1) component) obs],
+           or [n1 = component], and then by Hfull,
+            [In (Cobservation Send (Cpremessage p n1) n0) obs].
+           And we can have an invariant saying any message that has a Send observation
+           in a protocol state is a protocol message.
+
+           How do we prove that [Sy] is a protocol state?
+
+           Hfull implies that [Cobservation Receive (Cpremessate p n1) n0] is stored in obs.
+           Not necessarily: it may also happen that [Cobservation Send (Cpremessage p n1) n0]
+           is stored in obs. But in both cases, [Cpremessage p n1] should be protocol, right?
+           
+           We have some invariant saying that all messages for which we have
+           a Receive observation in obs satisfy isProtocol.
+
+           But do we have a Receive observation for [Cpremessage p n1] ?
+           
+         *)
+
+        assert(Hin' : n1 = component ->
+                     In (Cobservation Send (Cpremessage p component) component)
+                        (observationsOf (st (component_to_index component)))).
+        {
+          intros. subst.
+          pose proof (Hin := fullNode_last_receive_self _ _ _ _ _ _ Hfull).
+          exact Hin.
+        }
+        
+        assert (Hmproto: protocol_message_prop free_composite_elmo (Cpremessage p n1)).
+        {
+          destruct (decide (n1 = component)).
+          + subst.
+            specialize (Hin' (eq_refl component)).
+            (* Maybe the state from which the protocol message is sent can reach st? *)
+            eapply has_send_observation_implies_is_protocol.
+            2: { apply Hin'. }
+            exact Hpsp.
+          + 
+            (*Check all_receive_observation_have_component_as_witness.
+            Check fullNode_last_receive_not_self.*)
+            apply nesym in n2.
+            pose proof (Hin := fullNode_last_receive_not_self _ _ _ _ _ _ _ n2 Hfull).
+            pose proof (Harsip := protocol_state_satisfies_all_received_satisfy_isprotocol_prop _ (component_to_index component) Hpsp).
+            unfold all_received_satisfy_isprotocol_prop in Harsip.
+            rewrite -> Forall_forall in Harsip.
+            rewrite Heqobs in Hin.
+            specialize (Harsip _ Hin).
+            simpl in Harsip. clear Hin.
+
+           (* Maybe the state from which [Cpremessage p n2] is sent can reach st? *)
+            eapply (has_receive_observation_implies_is_protocol _ _ _ Hpsp).
+            eapply fullNode_last_receive_not_self.
+            2: { rewrite Heqobs in Hfull.
+                 rewrite -[component]component_to_index_to_component in Hfull.
+                 exact Hcomval.
+                 rewrite index_to_component_to_index in Hfull.
+                 apply Hfull.
+            }
+ 
+            
+            erewrite -> component_to_index_to_component.
+            exact n2.
+            exact Hcomval.
+        }
+        (* We have a protocol state Sy such that [Sy (component_to_index n) = Cprestate l]. *)
+        pose proof (Htmp := protocol_message_was_sent_from_protocol_state _ _ _ Hs).
+        destruct Htmp as [[Sy [Hsyproto Hsyn]] Hin''].
+        (* Maybe s0 is reachable from Sy ? *)
+
+        (* When the component [n] receives [Cpremessage p n1] in [Sy], the result is some state [Sx]
+           satisfying [Sx (component_to_index n)
+                       = (Cprestate (l ++ [Cobservation Receive (Cpremessage p n1) n0]))].
+         *)
+        destruct Hsyproto as [omSy Hsyproto].
+        destruct Hmproto as [_sm Hmproto].
+        (* Maybe _sm can reach st? *)
+        pose proof (Hgen := protocol_generated free_composite_elmo (existT _ (component_to_index n) Receive) _ _ Hsyproto _ _ Hmproto).
+        (* TODO how do we know the message is valid in the state? *)
+        unfold valid in Hgen. simpl in Hgen.
+        unfold constrained_composite_valid in Hgen. unfold free_constraint in Hgen. simpl in Hgen.
+        unfold vvalid in Hgen. simpl in Hgen.
+        rewrite Hsyn in Hgen. simpl in Hgen.
+        rewrite component_to_index_to_component in Hgen.
+        { exact Haddr. }
+        
+        assert (Hfn: fullNode (Cpremessage p n1) l n).
+        {
+          destruct (decide (n1 = n)).
+          2: { eapply isProtocol_last_fullNode. exact n2. apply Hproto'. }
+          subst n1.
+          (* Now: thanks to Hproto, we have [In (Cobservation Send (Cpremessage p n) n) l].
+             And an invariant should hold that for all 'send' observations, fullNode holds
+             (with the prefix). And (3), the prefix is a prefix of [l].
+           *)
+          pose proof (Hinp := isProtocol_last_sendInPrefix _ _ _ _ Hproto').
+          pose proof (Hfn := sent_is_fullNode).
+          specialize (Hfn Sy (Cpremessage p n)).
+          specialize (Hfn n n Haddr).
+          unfold protocol_state_prop in Hfn.
+          specialize (Hfn (@ex_intro _ _ omSy Hsyproto)).
+          simpl in Hfn.
+          specialize (Hfn (eq_refl n)).
+          rewrite Hsyn in Hfn.
+          simpl in Hfn.
+          specialize (Hfn Hinp).
+          exact Hfn.
+          (*
+          Print ex_intro.
+          Check sent_is_protocol.
+          epose proof (Hpmp := sent_is_protocol _ _ _ Haddr).
+          
+          epose proof (Hpmp := sent_is_protocol _ _ _ Haddr Hpsp).
+          specialize (Hpmp Hinp).
+          Search fullNode.
+          Check fullNode_appone.
+          pose proof (Hfull' := fullNode_appone _ _ _ _ _ Hfull).
+          Search obs. Search _sm.
+          *)
+        }
+        inversion Hfn. rewrite H1 in Hgen.
+        Check protocol_message_has_valid_sender.
+        pose proof (Haddr' := protocol_message_has_valid_sender _ _ (@ex_intro _ _ _sm Hmproto)).
+        assert (Hain : bool_decide (In n1 addresses) = true).
+        {
+          unfold address_valid in Haddr'.
+          assert (In n1 (seq 0 (length indices))).
+          { apply in_seq. split; lia. }
+          apply bool_decide_eq_true. exact H.
+        }
+        rewrite Hain in Hgen. simpl in Hgen. clear Haddr' Hain H1.
+        (* How to prove the non-self-equivocation check in Hgen?
+           By [Hmproto] we know that [Cpremessage p n] is protocol (in the composite);
+           therefore, it must have been sent by the node [n], and therefore
+           [n] should have its Send observation in the state (that is, in [l]).
+         *)
+
+        assert (n1 = n -> In (Cobservation Send (Cpremessage p n1) n) l).
+        { intros. subst n1. eapply isProtocol_last_receive_impl_send. apply Hproto'. }
+        assert ((if is_left (decide (n1 = n))
+          then bool_decide (In (Cobservation Send (Cpremessage p n1) n) l)
+                 else true) = true).
+        { destruct (decide (n1 = n)); simpl. subst.
+          apply bool_decide_eq_true. apply H. reflexivity. reflexivity. }
+        rewrite H1 in Hgen. simpl in Hgen. clear H H1.
+
+        rewrite HnoEquivCheck in Hgen.
+        assert (isProtocol p n1 weights None).
+        {
+          Check protocol_state_contains_receive_implies_isProtocol.
+          Search In isProtocol.
+        }
+        
+                                                         
+        
+        (*
+        Check protocol_state_contains_receive_implies_isProtocol.
+        Check has_send_observation_implies_is_protocol.
+        Search obs.*)
+
+        
+        (* [om] is [Some _]. Or not? *)
+        destruct om.
+        2: {
+          unfold vtransition in H0.
+          simpl in H0.
+          destruct v.
+          { inversion H0. }
+          inversion H0. subst.
+          rewrite H2 in H0. simpl in H0.
+        }
+        
+        subst. clear H0.
+        simpl in Hs.
+        simpl in IHl.
+        (* Now [Cprestate l] is a protocol state (see the hypothesis Hps) *)
+        (* We also need the message [Cpremessage p n1] to be protocol;
+         the we can prove that [Cprestate (l :: Cobservation Receive (Cpremessage p n1) n0)]
+         is also a protocol state.
+
+         Hproto' means that the 'current' node [n] can receive the big message.
+         I would need to have
+         *)
+        Print protocol_prop.
+
+
+        (*
+      assert (n0 = n).
+      { unfold isProtocol in Hproto'.
+        simpl in Hproto'.
+        rewrite fold_left_app in Hproto'.
+        simpl in Hproto'.
+      }
+         *)
+        
+        Print elmo_vlsm_machine.
+        (*remember (mk_vlsm (elmo_vlsm_machine n weights treshold)) as X.*)
+        simpl.
+        Print protocol_prop.
+        pose proof (Hnext := protocol_generated (mk_vlsm (elmo_vlsm_machine n weights treshold)) Receive (Cprestate l) _om Hps).
+        Print protocol_message_prop.
+        Search protocol_message_prop.
+  Abort.
+
+  
+  Context
+        (i : index)
+        (Xi := composite_vlsm_constrained_projection IM composition_constraint i)
+  .
+  
+  
+  Theorem elmo_validating:
+    validating_projection_prop IM composition_constraint i.
+  Proof.
+    intros li siomi H.
+    unfold protocol_valid in H.
+    unfold vvalid. unfold valid. unfold machine. simpl.
+    unfold projection_valid.
+    destruct siomi as [si omi].
+    destruct H as [Hpsp [Hopmp Hvalid]].
+    unfold valid in Hvalid. unfold machine in Hvalid. simpl in Hvalid. unfold IM in Hvalid.
+    unfold IM' in Hvalid. inversion Hvalid.
+    unfold vvalid in Hvalid.
+  Abort.
+  
+
+
+End composition.
